truth table implementation lib WIP

books/centaur/truth/dsd4-aignet.lisp
@@ -35,6 +35,9 @@
 (include-book "tools/symlet" :dir :system)
 (include-book "centaur/fty/deftypes" :dir :system)
 (include-book "centaur/aignet/construction" :dir :system)
+(include-book "centaur/aignet/mark-impls" :dir :system)
+(include-book "centaur/aignet/statsmgr" :dir :system)
+
 
 (local (include-book "tools/trivial-ancestors-check" :dir :system))
 (local (include-book "centaur/bitops/ihsext-basics" :dir :system))
@@ -488,7 +491,7 @@
                                     aignet)
   :guard (and (only-depends-on x indices 4)
               (<= 4 (aignet::num-ins aignet)))
-  :returns (mv (lit aignet::litp)
+  :returns (mv (lit aignet::litp :rule-classes :type-prescription)
                (new-strash)
                (new-aignet))
   :measure (len indices)
@@ -595,6 +598,7 @@
     :hints(("Goal" :in-theory (enable only-depends-on)))))
 
 
+
 (defines aignet-build-truth4-decomp-single
   :prepwork ((local
               (defthm depends-on-when-positive-cofactor-not-equal-x
@@ -608,7 +612,7 @@
                                                  (full-indices (and (index-listp full-indices 4)
                                                                (full-perm-p full-indices 4))))
     :returns (mv successp
-                 (lit aignet::litp)
+                 (lit aignet::litp :rule-classes :type-prescription)
                  (new-strash)
                  (new-aignet))
     :guard (and (< n 4)
@@ -678,7 +682,7 @@
                                                                      (full-perm-p full-indices 4))))
     :guard (<= 4 (aignet::num-ins aignet))
     :measure (list (count-truth4-deps x) (+ 1 (len full-indices)))
-    :returns (mv (lit aignet::litp)
+    :returns (mv (lit aignet::litp :rule-classes :type-prescription)
                  (new-strash)
                  (new-aignet))
     (b* (((mv ok lit strash aignet)
@@ -695,7 +699,7 @@
     :guard (<= 4 (aignet::num-ins aignet))
     :measure (list (count-truth4-deps x) (len indices))
     :returns (mv (successp)
-                 (lit aignet::litp)
+                 (lit aignet::litp :rule-classes :type-prescription)
                  (new-strash)
                  (new-aignet))
     (b* (((when (atom indices))
@@ -976,7 +980,7 @@
                                         (full-indices (and (index-listp full-indices 4)
                                                            (full-perm-p full-indices 4))))
   :returns (mv success
-               (lit aignet::litp)
+               (lit aignet::litp :rule-classes :type-prescription)
                (new-strash)
                (new-aignet))
   :guard (and (< n 4) (< m 4)
@@ -1310,7 +1314,7 @@
   :guard (and (< n 4)
               (<= 4 (num-ins aignet)))
   :returns (mv (successp)
-               (lit aignet::litp)
+               (lit aignet::litp :rule-classes :type-prescription)
                (new-strash)
                (new-aignet))
   :well-founded-relation acl2::nat-list-<
@@ -1367,7 +1371,7 @@
   :guard (and (<= 4 (num-ins aignet))
               (consp indices))
   :returns (mv (successp)
-               (lit aignet::litp)
+               (lit aignet::litp :rule-classes :type-prescription)
                (new-strash)
                (new-aignet))
   :well-founded-relation acl2::nat-list-<
@@ -1409,25 +1413,77 @@
     :hints (("goal" :induct t :expand ((index-listp indices 4))))))
 
 
+(aignet::defstatsmgr dsd4stats
+  (simple)
+  (single)
+  (double)
+  (both)
+  (node-simple)
+  (node-single)
+  (node-double)
+  (node-both))
+
+(define dsd4stats-snap (dsd4stats)
+  :returns (lst eqlable-listp)
+  (list (lnfix (dsd4stats-simple dsd4stats))
+        (lnfix (dsd4stats-single dsd4stats))
+        (lnfix (dsd4stats-double dsd4stats))
+        (lnfix (dsd4stats-both dsd4stats))))
+
+(define dsd4stats-node-count ((snap eqlable-listp) dsd4stats)
+  (b* (((list ssimple ssingle sdouble sboth) snap)
+       (dsd4stats (incr-dsd4stats-node-simple-cond (not (eql ssimple (dsd4stats-simple dsd4stats))) dsd4stats))
+       (dsd4stats (incr-dsd4stats-node-single-cond (not (eql ssingle (dsd4stats-single dsd4stats))) dsd4stats))
+       (dsd4stats (incr-dsd4stats-node-double-cond (not (eql sdouble (dsd4stats-double dsd4stats))) dsd4stats))
+       (dsd4stats (incr-dsd4stats-node-both-cond (not (eql sboth (dsd4stats-both dsd4stats))) dsd4stats)))
+    dsd4stats))
+
+(define dsd4stats-count (single-ok double-ok dsd4stats)
+  (if single-ok
+      (if double-ok
+          (incr-dsd4stats-both dsd4stats)
+        (incr-dsd4stats-single dsd4stats))
+    (if double-ok
+        (incr-dsd4stats-double dsd4stats)
+      (incr-dsd4stats-simple dsd4stats))))
+
 (define aignet-build-truth4-decomp ((x truth4-p)
                                     strash
                                     aignet
+                                    dsd4stats
                                     (full-indices (and (index-listp full-indices 4)
                                                        (full-perm-p full-indices 4))))
-  :returns (mv (lit aignet::litp)
+  :returns (mv (lits aignet::lit-listp)
                (new-strash)
-               (new-aignet))
+               (new-aignet)
+               (new-dsd4stats))
   :guard (<= 4 (num-ins aignet))
-  (b* ((num-deps (count-truth4-deps x))
-       ((when (< num-deps 4))
-        (aignet-build-truth4-decomp-single-or-simple x strash aignet full-indices))
-       ((mv simple-ok lit strash aignet)
+  ;; (b* ((num-deps (count-truth4-deps x))
+  ;;      ((when (< num-deps 4))
+  ;;       (aignet-build-truth4-decomp-single-or-simple x strash aignet full-indices))
+  ;;      ((mv simple-ok lit strash aignet)
+  ;;       (aignet-build-truth4-decomp-single full-indices x strash aignet full-indices))
+  ;;      ((when simple-ok) (mv lit strash aignet))
+  ;;      ((mv nonsimple-ok lit strash aignet)
+  ;;       (aignet-build-truth4-decomp-rec full-indices x strash aignet full-indices))
+  ;;      ((when nonsimple-ok) (mv lit strash aignet)))
+  ;;   (aignet-build-truth4-simple full-indices x strash aignet))
+  (b* (;; (num-deps (count-truth4-deps x))
+       ((mv single-ok single-lit strash aignet)
         (aignet-build-truth4-decomp-single full-indices x strash aignet full-indices))
-       ((when simple-ok) (mv lit strash aignet))
-       ((mv nonsimple-ok lit strash aignet)
+       ((mv double-ok double-lit strash aignet)
         (aignet-build-truth4-decomp-rec full-indices x strash aignet full-indices))
-       ((when nonsimple-ok) (mv lit strash aignet)))
-    (aignet-build-truth4-simple full-indices x strash aignet))
+       (dsd4stats (dsd4stats-count single-ok double-ok dsd4stats)))
+    (if single-ok
+        (if (and double-ok
+                 (not (eql single-lit double-lit)))
+            (mv (list single-lit double-lit) strash aignet dsd4stats)
+          (mv (list single-lit) strash aignet dsd4stats))
+      (if double-ok
+          (mv (list double-lit) strash aignet dsd4stats)
+        (b* (((mv simple-lit strash aignet)
+              (aignet-build-truth4-simple full-indices x strash aignet)))
+          (mv (list simple-lit) strash aignet dsd4stats)))))
   ///
   
   (aignet::def-aignet-preservation-thms aignet-build-truth4-decomp :stobjname aignet)
@@ -1440,17 +1496,40 @@
                (equal (stype-count stype new-aignet)
                       (stype-count stype aignet)))))
 
-  (defret aignet-litp-of-aignet-build-truth4-decomp
+  (defret aignet-lit-listp-of-aignet-build-truth4-decomp
     (implies (and (<= 4 (aignet::num-ins aignet))
                   (index-listp full-indices 4))
+             (aignet::aignet-lit-listp lits new-aignet)))
+
+  (defret aignet-litp-member-of-aignet-build-truth4-decomp
+    (implies (and (member lit lits)
+                  (index-listp full-indices 4)
+                  (<= 4 (aignet::num-ins aignet)))
              (aignet::aignet-litp lit new-aignet)))
 
-  (defret lit-eval-of-aignet-build-truth4-decomp
-    (implies (and (<= 4 (aignet::num-ins aignet))
+  (defret eval-member-of-aignet-build-truth4-decomp
+    (implies (and (member lit lits)
                   (index-listp full-indices 4)
-                  (full-perm-p full-indices 4))
+                  (full-perm-p full-indices 4)
+                  (<= 4 (aignet::num-ins aignet)))
              (equal (aignet::lit-eval lit invals regvals new-aignet)
-                    (bool->bit (truth-eval x (truth4-env-from-aignet-invals invals) 4))))))
+                    (bool->bit (truth-eval x (truth4-env-from-aignet-invals invals) 4)))))
+
+  (defret true-listp-of-aignet-build-truth4-decomp
+    (true-listp lits) :rule-classes :type-prescription)
+
+  ;; (defret aignet-litp-of-aignet-build-truth4-decomp
+  ;;   (implies (and (<= 4 (aignet::num-ins aignet))
+  ;;                 (index-listp full-indices 4))
+  ;;            (aignet::aignet-litp lit new-aignet)))
+
+  ;; (defret lit-eval-of-aignet-build-truth4-decomp
+  ;;   (implies (and (<= 4 (aignet::num-ins aignet))
+  ;;                 (index-listp full-indices 4)
+  ;;                 (full-perm-p full-indices 4))
+  ;;            (equal (aignet::lit-eval lit invals regvals new-aignet)
+  ;;                   (bool->bit (truth-eval x (truth4-env-from-aignet-invals invals) 4)))))
+  )
 
 (fty::deflist truth4-list :elt-type truth4)
 
@@ -1462,24 +1541,39 @@
          (full-perm-p (car x) 4)
          (permutations4p (cdr x)))))
 
+(local (defthm lit-listp-of-append
+         (implies (and (aignet::lit-listp x)
+                       (aignet::lit-listp y))
+                  (aignet::lit-listp (append x y)))
+         :hints(("Goal" :in-theory (enable append)))))
 
+(local (defthm aignet-lit-listp-of-append
+         (implies (and (aignet::aignet-lit-listp x aignet)
+                       (aignet::aignet-lit-listp y aignet))
+                  (aignet::aignet-lit-listp (append x y) aignet))
+         :hints(("Goal" :in-theory (enable append)))))
 
+(local (defthm member-append
+         (iff (member x (append a b))
+              (or (member x a) (member x b)))))
 
 (define aignet-build-truth4-decomp-perms ((x truth4-p)
                                           (perms permutations4p)
                                           strash
-                                          aignet)
+                                          aignet
+                                          dsd4stats)
   :returns (mv (lits aignet::lit-listp)
                (new-strash)
-               (new-aignet))
+               (new-aignet)
+               (new-dsd4stats))
   :guard (<= 4 (num-ins aignet))  
   :verify-guards nil
-  (b* (((when (atom perms)) (mv nil strash aignet))
-       ((mv lit1 strash aignet)
-        (aignet-build-truth4-decomp x strash aignet (car perms)))
-       ((mv rest strash aignet)
-        (aignet-build-truth4-decomp-perms x (cdr perms) strash aignet)))
-    (mv (cons lit1 rest) strash aignet))
+  (b* (((when (atom perms)) (mv nil strash aignet dsd4stats))
+       ((mv lits1 strash aignet dsd4stats)
+        (aignet-build-truth4-decomp x strash aignet dsd4stats (car perms)))
+       ((mv rest strash aignet dsd4stats)
+        (aignet-build-truth4-decomp-perms x (cdr perms) strash aignet dsd4stats)))
+    (mv (append lits1 rest) strash aignet dsd4stats))
   ///
 
   (aignet::def-aignet-preservation-thms aignet-build-truth4-decomp-perms :stobjname aignet)
@@ -1683,7 +1777,6 @@
                  (2 (perm4-perm-index2 x))
                  (t (perm4-perm-index3 x)))))
 
-
 )
 
 (define perm4-to-index-list ((x perm4p))
@@ -1860,29 +1953,33 @@
                                         (truth4arr)
                                         (smm "storage for output literals")
                                         strash
-                                        aignet)
+                                        aignet
+                                        dsd4stats)
   :guard (and (<= (acl2::smm-nblocks smm) canonical-count)
               (<= canonical-count (truth4s-length truth4arr))
               (<= 4 (num-ins aignet)))
   :measure (nfix (- (nfix canonical-count) (acl2::smm-nblocks smm)))
-  :returns (mv new-smm new-strash new-aignet)
+  :returns (mv new-smm new-strash new-aignet new-dsd4stats)
   :prepwork ((local (defthm eqlable-listp-when-lit-listp
                       (implies (aignet::lit-listp x)
                                (eqlable-listp x)))))
   (b* ((n (acl2::smm-nblocks smm))
        ((when (mbe :logic (zp (- (nfix canonical-count) n))
                    :exec (eql n canonical-count)))
-        (mv smm strash aignet))
+        (mv smm strash aignet dsd4stats))
        (truth (get-truth4 n truth4arr))
-       ((mv lits strash aignet)
+       (snap (dsd4stats-snap dsd4stats))
+       ((mv lits strash aignet dsd4stats)
         (aignet-build-truth4-decomp-perms truth
                                           (all-permutations4)
                                           strash
-                                          aignet))
+                                          aignet
+                                          dsd4stats))
+       (dsd4stats (dsd4stats-node-count snap dsd4stats))
        (lits (remove-duplicates lits))
        (smm (acl2::smm-addblock (len lits) smm))
        (smm (smm-write-lits n 0 lits smm)))
-    (aignet-build-truth4arr-decomps canonical-count truth4arr smm strash aignet))
+    (aignet-build-truth4arr-decomps canonical-count truth4arr smm strash aignet dsd4stats))
   ///
   (defret smm-nblocks-of-aignet-build-truth4arr-decomps
     (implies (<= (len smm) (nfix canonical-count))
@@ -1947,15 +2044,20 @@
                                             aignet)
   :returns (mv new-smm new-aignet)
   :guard (<= canonical-count (truth4s-length truth4arr))
-  (b* (((acl2::local-stobjs strash)
-        (mv smm strash aignet))
+  (b* (((acl2::local-stobjs strash dsd4stats)
+        (mv smm strash aignet dsd4stats))
        (aignet (aignet::aignet-init 0 0 4 5000 aignet))
        (aignet (aignet::aignet-add-in aignet))
        (aignet (aignet::aignet-add-in aignet))
        (aignet (aignet::aignet-add-in aignet))
        (aignet (aignet::aignet-add-in aignet))
-       (smm (smm-clear smm)))
-    (aignet-build-truth4arr-decomps canonical-count truth4arr smm strash aignet))
+       (smm (smm-clear smm))
+       ((mv smm strash aignet dsd4stats)
+        (aignet-build-truth4arr-decomps canonical-count truth4arr smm strash aignet dsd4stats)))
+    (print-dsd4stats dsd4stats)
+    (mv smm strash aignet dsd4stats))
+       
+    
   ///
   
   (defret smm-nblocks-of-aignet-build-truth4arr-decomps-top
@@ -2054,22 +2156,10 @@
 
 
 (defstobj dsdlib
-  (npns :type npn4arr)
-  (truths :type truth4arr)
-  (aigs :type aignet)
-  (cands :type smm)
-  :renaming ((npns dsdlib->npns)
-             (update-npns update-dsdlib->npns)
-             (npnsp dsdlib-npns-p)
-             (truths dsdlib->truths)
-             (update-truths update-dsdlib->truths)
-             (truthsp dsdlib-truths-p)
-             (aigs dsdlib->aigs)
-             (update-aigs update-dsdlib->aigs)
-             (aigsp dsdlib-aigs-p)
-             (cands dsdlib->cands)
-             (update-cands update-dsdlib->cands)
-             (candsp dsdlib-cands-p)))
+  (dsdlib->npns :type npn4arr)
+  (dsdlib->truths :type truth4arr)
+  (dsdlib->aigs :type aignet)
+  (dsdlib->cands :type smm))
 
 (include-book "std/stobjs/nested-stobjs" :dir :system)
 
@@ -2232,7 +2322,28 @@
                    (npn (nth truth (dsdlib->npns dsdlib)))
                    (truth (nth (npn4->truth-idx (nth truth (dsdlib->npns dsdlib)))
                                (dsdlib->truths dsdlib)))
-                   (orig-env (truth4-env-from-aignet-invals invals))))))))
+                   (orig-env (truth4-env-from-aignet-invals invals)))))))
+
+  (defthm dsdlib-correct-implies-id-eval-smm-lookup-of-truth-idx
+    (b* ((?truth4arr (dsdlib->truths dsdlib))
+         (aignet (dsdlib->aigs dsdlib))
+         (smm (dsdlib->cands dsdlib))
+         (npn4arr (dsdlib->npns dsdlib))
+         ((npn4 npn) (nth truth npn4arr))
+         (env (permuted-env-from-aignet-invals npn invals)))
+      (implies (and (dsdlib-correct dsdlib)
+                    (dsdlib-wfp dsdlib)
+                    (truth4-p truth)
+                    (< (nfix idx) (len (nth npn.truth-idx smm))))
+               (equal (aignet::id-eval (aignet::lit-id (nth idx (nth npn.truth-idx smm))) invals regvals aignet)
+                      (b-xor (aignet::lit-neg (nth idx (nth npn.truth-idx smm)))
+                             (b-xor npn.negate
+                                    (bool->bit (truth-eval truth env 4)))))))
+    :hints (("goal" :use dsdlib-correct-implies-eval-smm-lookup-of-truth-idx
+             :in-theory (e/d (aignet::lit-eval b-xor bool->bit)
+                             (dsdlib-correct
+                              dsdlib-correct-implies-eval-smm-lookup-of-truth-idx
+                              dsdlib-correct-implies-eval-smm-lookup))))))
                
              
 
@@ -2256,8 +2367,2135 @@
     (dsdlib-correct initialized-dsdlib)
     :hints(("Goal" :in-theory (enable dsdlib-correct)))))
 
-(local (in-theory (disable dsdlib->npns
-                           dsdlib->cands
-                           dsdlib->aigs
-                           dsdlib->truths)))
+(defthm dsdlibp-implies
+  (implies (dsdlibp dsdlib)
+           (and (npn4arrp (dsdlib->npns dsdlib))
+                (truth4arrp (dsdlib->truths dsdlib))
+                (aignet::node-listp (dsdlib->aigs dsdlib))
+                (aignet::aignet-nodes-ok (dsdlib->aigs dsdlib))
+                (acl2::u32-list-listp (dsdlib->cands dsdlib)))))
 
+(in-theory (disable dsdlibp
+                    dsdlib->npns
+                    dsdlib->cands
+                    dsdlib->aigs
+                    dsdlib->truths))
+
+(define dsdlib-num-nodes (dsdlib)
+  :enabled t
+  (stobj-let
+   ((aignet (dsdlib->aigs dsdlib)))
+   (count)
+   (num-nodes aignet)
+   count))
+
+(define dsdlib-num-cands (dsdlib)
+  :enabled t
+  (stobj-let
+   ((smm (dsdlib->cands dsdlib)))
+   (count)
+   (smm-max-index smm)
+   count))
+
+"AIGNET"
+
+;; (depends-on "abcdata.lsp")
+(make-event
+ (b* (((mv err val state)
+       (acl2::read-file "abcdata.lsp" state))
+      ((when err)
+       (er hard? '*abcdata* "Couldn't read abcdata.lsp")
+       (mv nil nil state))
+      ((unless (eql (len val) 3))
+       (er hard? '*abcdata* "abcdata.lsp should contain 3 objects but found ~x0" (len val))
+       (mv nil nil state)))
+   (value `(defconst *abcdata* ',val))))
+
+(defconst *abc-nodes* (cdr (assoc :nodedata *abcdata*)))
+(defconst *abc-outs* (cdr (assoc :outdata *abcdata*)))
+(defconst *abc-prios* (cdr (assoc :priodata *abcdata*)))
+
+
+
+
+#!truth
+(defmacro lit-truth (lit t4arr)
+  `(truth-norm4 (logxor (- (aignet::lit-neg ,lit))
+                        (get-truth4 (aignet::lit-id ,lit) ,t4arr))))
+
+(defstobj-clone truth4arr truth::truth4arr :strsubst (("a" . "a")))
+
+
+(define abc-nodes-wellformed ((num-nodes natp)
+                              (nodedata nat-listp))
+  :measure (len nodedata)
+  (if (atom nodedata)
+      t
+    (and (consp (cdr nodedata))
+         (< (lit->var (car nodedata)) (lnfix num-nodes))
+         (< (lit->var (cadr nodedata)) (lnfix num-nodes))
+         (abc-nodes-wellformed (+ 1 (lnfix num-nodes)) (cddr nodedata)))))
+
+(define aignet-build-abc-nodes ((nodes nat-listp) aignet)
+  :guard (and (not (equal 0 (num-nodes aignet)))
+              (abc-nodes-wellformed (+ -1 (num-nodes aignet)) nodes)
+              (equal (num-outs aignet) 0)
+              (equal (num-nxsts aignet) 0))
+  :guard-hints (("goal" :expand ((abc-nodes-wellformed (node-count aignet) nodes))))
+
+  :prepwork ((local (defthm no-outputs-when-no-outputs
+                      (implies (and (equal (stype-count :po aignet) 0)
+                                    (equal (stype-count :nxst aignet) 0))
+                               (not (equal (ctype (stype (car (lookup-id n aignet)))) :output)))
+                      :hints(("Goal" :in-theory (enable lookup-id stype-count)
+                              :induct t)
+                             (and stable-under-simplificationp
+                                  '(:in-theory (enable ctype))))))
+             (local (defthm aignet-litp-when-no-outs
+                      (implies (and (equal (stype-count :po aignet) 0)
+                                    (equal (stype-count :nxst aignet) 0))
+                               (iff (aignet-litp lit aignet)
+                                    (< (lit-id lit) (num-nodes aignet))))
+                      :hints(("Goal" :in-theory (enable aignet-litp))))))
+
+  :returns (new-aignet)
+  (b* (((when (atom nodes)) aignet)
+       ((list fanin0 fanin1) nodes)
+       (lit0 (make-lit (+ 1 (lit->var fanin0)) (lit->neg fanin0)))
+       (lit1 (make-lit (+ 1 (lit->var fanin1)) (lit->neg fanin1)))
+       (aignet (aignet-add-gate lit0 lit1 aignet)))
+    (aignet-build-abc-nodes (cddr nodes) aignet)))
+
+(define aignet-build-abc-top (aignet)
+  :returns (new-aignet)
+  (b* ((node-data *abc-nodes*)
+       (aignet (aignet-init 0 0 4 (+ 5 (/ (len node-data) 2)) aignet))
+       (aignet (aignet-add-in aignet))
+       (aignet (aignet-add-in aignet))
+       (aignet (aignet-add-in aignet))
+       (aignet (aignet-add-in aignet)))
+    (aignet-build-abc-nodes node-data aignet)))
+
+(define aignet-derive-truth4s ((n natp)
+                               (aignet)
+                               (truth4arr))
+  :guard (and (<= (num-nodes aignet) (truth4s-length truth4arr))
+              (<= (num-ins aignet) 4)
+              (equal 0 (num-regs aignet))
+              (<= n (num-nodes aignet)))
+  :measure (nfix (- (num-nodes aignet) (nfix n)))
+  :returns (new-truth4arr)
+  :guard-hints (("goal" :in-theory (enable aignet-idp)))
+  :prepwork ((local (defthm unsigned-byte-p-when-truth4-p
+                      (implies (truth::truth4-p x)
+                               (unsigned-byte-p 16 x))
+                      :hints(("Goal" :in-theory (enable truth::truth4-p)))))
+             (local (defthm stype-when-ctype-input
+                      (implies (equal 0 (stype-count :reg aignet))
+                               (equal (equal (ctype (stype (car aignet))) :input)
+                                      (equal (stype (car aignet)) :pi)))
+                      :hints(("Goal" :in-theory (enable ctype))))))
+  (b* (((when (mbe :logic (zp (- (num-nodes aignet) (nfix n)))
+                   :exec (eql n (num-nodes aignet))))
+        truth4arr)
+       (type (id->type n aignet))
+       (truth4arr
+        (aignet-case type
+          :in (b* ((truth (truth::var4 (io-id->ionum n aignet))))
+                (set-truth4 n truth truth4arr))
+          :gate (b* ((lit0 (gate-id->fanin0 n aignet))
+                     (lit1 (gate-id->fanin1 n aignet)))
+                  (set-truth4 n (logand (truth::lit-truth lit0 truth4arr)
+                                        (truth::lit-truth lit1 truth4arr))
+                              truth4arr))
+          :out (b* ((lit (co-id->fanin n aignet)))
+                 (set-truth4 n (truth::lit-truth lit truth4arr)
+                             truth4arr))
+          :const (set-truth4 n 0 truth4arr))))
+    (aignet-derive-truth4s (1+ (lnfix n)) aignet truth4arr))
+  ///
+  (local (defun-sk truths-ok (n truth4arr aignet invals regvals)
+           (forall id
+                   (implies (< (nfix id) (nfix n))
+                            (equal (id-eval id invals regvals aignet)
+                                   (bool->bit (truth::truth-eval
+                                               (nth id truth4arr)
+                                               (truth::truth4-env-from-aignet-invals invals) 4)))))
+           :rewrite :direct))
+  (local (in-theory (disable truths-ok)))
+
+  (local (defthm truth-eval-of-minus-bit
+           (implies (bitp x)
+                    (equal (truth::truth-eval (- x) env numvars)
+                           (acl2::bit->bool x)))
+           :hints(("Goal" :in-theory (enable truth::truth-eval)))))
+
+  (local (in-theory (e/d* (acl2::arith-equiv-forwarding)
+                          (acl2::nfix-equal-to-nonzero))))
+
+  (local (defret truths-ok-of-aignet-derive-truth4s
+           (implies (and (truths-ok n truth4arr aignet invals regvals)
+                         (equal (stype-count :reg aignet) 0)
+                         (<= (stype-count :pi aignet) 4))
+                    (truths-ok (+ 1 (node-count aignet))
+                               new-truth4arr aignet invals regvals))
+           :hints (("goal" :induct <call> :expand (<call>))
+                   (and stable-under-simplificationp
+                        (let ((lit (assoc 'truths-ok clause)))
+                          (and lit
+                               `(:expand (,lit)))))
+                   (and stable-under-simplificationp
+                        '(:expand ((id-eval n invals regvals aignet))
+                          :in-theory (enable eval-and-of-lits lit-eval))))))
+
+  (local (defthm truths-ok-of-0
+           (truths-ok 0 truth4arr aignet invals regvals)
+           :hints(("Goal" :in-theory (enable truths-ok)))))
+
+  (defthm aignet-derive-truth4s-correct
+    (b* ((new-truth4arr (aignet-derive-truth4s 0 aignet truth4arr)))
+      (implies (and (equal (stype-count :reg aignet) 0)
+                    (<= (stype-count :pi aignet) 4)
+                    (< (nfix id) (num-nodes aignet)))
+             (equal (truth::truth-eval
+                     (nth id new-truth4arr)
+                     (truth::truth4-env-from-aignet-invals invals)
+                     4)
+                    (acl2::bit->bool (id-eval id invals nil aignet)))))
+    :hints (("goal" :use ((:instance truths-ok-of-aignet-derive-truth4s
+                           (n 0) (regvals nil)))
+             :in-theory (disable truths-ok-of-aignet-derive-truth4s)))))
+
+(define collect-id-truths ((x nat-listp)
+                           truth4arr)
+  (if (atom x)
+      nil
+    (cons (and (< (lnfix (car x)) (truth4s-length truth4arr))
+               (get-truth4 (car x) truth4arr))
+          (collect-id-truths (cdr x) truth4arr))))
+
+(define truths-negnorm ((x nat-listp))
+  (if (atom x)
+      nil
+    (b* ((xnorm (truth::truth-norm4 (car x))))
+      (cons (if (< xnorm (truth::truth-norm4 (lognot xnorm)))
+                xnorm
+              (truth::truth-norm4 (lognot xnorm)))
+            (truths-negnorm (cdr x))))))
+
+(define incr-ids ((x nat-listp))
+  (if (atom x)
+      nil
+    (cons (+ 1 (lnfix (car x)))
+          (incr-ids (cdr x)))))
+             
+
+
+       
+
+
+(define setup-dsd4-lib-abc (npn4arr
+                            truth4arr
+                            aignet
+                            smm) ;; all emptied
+  :returns (mv new-npn4arr
+               new-truth4arr
+               new-smm
+               new-aignet)
+  (b* (((mv count npn4arr truth4arr) (record-all-npn4-perms-top npn4arr truth4arr))
+       ((mv smm aignet) (aignet-build-abc-lib truth4arr aignet smm)))
+    (mv npn4arr truth4arr smm aignet))
+  ///
+  (defret npn4arr-length-of-setup-dsd4-lib-abc
+    (equal (len new-npn4arr) #x10000))
+
+  (defret npn4arr-indices-bounded-of-setup-dsd4-lib-abc
+    (npn4arr-indices-bounded (len new-smm) new-npn4arr))
+
+  (defret npn4arr-correct-of-setup-dsd4-lib-abc
+    (npn4arr-correct new-npn4arr new-truth4arr))
+
+  (defret num-ins-of-setup-dsd4-lib-abc-aignet
+    (equal (aignet::stype-count :pi new-aignet) 4))
+
+  (defret aignet-litp-smm-lookup-of-setup-dsd4-lib-abc
+    (implies (and (< (nfix n) (len new-smm))
+                  (< (nfix idx) (len (nth n new-smm))))
+             (aignet::aignet-litp (nth idx (nth n new-smm)) new-aignet))
+    :hints(("Goal" :in-theory (enable* acl2::arith-equiv-forwarding))))
+
+  (defret smm-contains-aignet-lits-of-setup-dsd4-lib-abc
+    (smm-contains-aignet-lits new-smm new-aignet)
+    :hints (("goal" :in-theory (e/d (smm-contains-aignet-lits) (setup-dsd4-lib-abc)))))
+
+  (defret truth4arr-length-of-setup-dsd4-lib-abc
+    (<= (len new-smm) (len new-truth4arr))
+    :rule-classes :linear)
+
+  (defret eval-smm-lookup-of-setup-dsd4-lib-abc
+    (implies (and (< (nfix n) (len new-smm))
+                  (< (nfix idx) (len (nth n new-smm))))
+             (equal (aignet::lit-eval (nth idx (nth n new-smm)) invals regvals new-aignet)
+                    (bool->bit (truth-eval (nth n new-truth4arr) (truth4-env-from-aignet-invals invals) 4))))
+    :hints(("Goal" :in-theory (enable* acl2::arith-equiv-forwarding))))
+
+  (defret dsd4-truth-impls-correct-of-setup-dsd4-lib-abc
+    (dsd4-truth-impls-correct new-smm new-aignet new-truth4arr)
+    :hints(("Goal" :in-theory (enable dsd4-truth-impls-correct))))
+
+  (defret npn4arr-indices-all-bound-of-setup-dsd4-lib-abc
+    (npn4arr-indices-all-bound new-npn4arr))))
+    
+
+
+
+
+"AIGNET"
+
+
+
+(defstobj-clone eba2 eba :suffix "2")
+(defstobj-clone smm acl2::smm :strsubst (("a" . "a")))
+
+
+
+(define aignet-count-gates-eba ((n natp)
+                          (eba)
+                          (aignet))
+  :guard (and (<= (nfix n) (max-fanin aignet))
+              (< (max-fanin aignet) (eba-length eba)))
+  :returns (mv (count natp :rule-classes :type-prescription)
+               new-eba)
+  :verify-guards nil
+  (b* (((when (eql (eba-get-bit n eba) 1)) (mv 0 eba))
+       (eba (eba-set-bit n eba))
+       (type (id->type n aignet)))
+    (aignet-case type
+      :out (aignet-count-gates-eba (lit-id (co-id->fanin n aignet)) eba aignet)
+      :gate (b* (((mv count1 eba) (aignet-count-gates-eba (lit-id (gate-id->fanin0 n aignet)) eba aignet))
+                 ((mv count2 eba) (aignet-count-gates-eba (lit-id (gate-id->fanin1 n aignet)) eba aignet)))
+              (mv (+ 1 count1 count2) eba))
+      :in (mv 0 eba)
+      :const (mv 0 eba)))
+  ///
+  (defret eba-length-of-aignet-count-gates-eba
+    (implies (and (< (max-fanin aignet) (len eba))
+                  (<= (nfix n) (max-fanin aignet)))
+             (equal (len new-eba) (len eba))))
+
+  (verify-guards aignet-count-gates-eba
+    :hints(("Goal" :in-theory (enable aignet-idp)))))
+
+
+(define aignet-mark-cone ((n natp)
+                          (eba)
+                          (aignet))
+  :guard (and (<= (nfix n) (max-fanin aignet))
+              (< (max-fanin aignet) (eba-length eba)))
+  :returns (new-eba)
+  :verify-guards nil
+  (b* (((when (eql (eba-get-bit n eba) 1)) eba)
+       (eba (eba-set-bit n eba))
+       (type (id->type n aignet)))
+    (aignet-case type
+      :out (aignet-mark-cone (lit-id (co-id->fanin n aignet)) eba aignet)
+      :gate (b* ((eba (aignet-mark-cone (lit-id (gate-id->fanin0 n aignet)) eba aignet)))
+              (aignet-mark-cone (lit-id (gate-id->fanin1 n aignet)) eba aignet))
+      :in eba
+      :const eba))
+  ///
+  (defret eba-length-of-aignet-mark-cone
+    (implies (and (< (max-fanin aignet) (len eba))
+                  (<= (nfix n) (max-fanin aignet)))
+             (equal (len new-eba) (len eba))))
+
+  (verify-guards aignet-mark-cone
+    :hints(("Goal" :in-theory (enable aignet-idp)))))
+
+
+
+(define smm-push-last ((val :type (unsigned-byte 32))
+                       (smm))
+  :guard (not (equal 0 (smm-nblocks smm)))
+  :prepwork ((local (in-theory (disable len resize-list)))
+             (local (include-book "std/lists/resize-list" :dir :system))
+             (local (include-book "std/lists/update-nth" :dir :system))
+             (local (defthm update-nth-of-len-resize
+                      (equal (update-nth (len x) val (resize-list x (+ 1 (len x)) default))
+                             (append x (list val)))
+                      :hints (("goal" :induct (len x)
+                               :in-theory (enable (:i len))
+                               :expand ((len x)
+                                        (:free (n val a b) (update-nth n val (cons a b)))
+                                        (:free (len) (resize-list x len default))))))))
+  :returns (new-smm)
+  (mbe :logic
+       (non-exec (update-nth (1- (len smm))
+                             (append (nth (1- (len smm)) smm) (list (nfix val)))
+                             smm))
+       :exec 
+       (b* ((last (1- (smm-nblocks smm)))
+            (last-sz (smm-block-size last smm))
+            (smm (smm-resize-last (+ 1 last-sz) smm)))
+         (smm-write last last-sz val smm)))
+  ///
+  (fty::deffixequiv smm-push-last :args ((val natp)))
+
+  (defret nth-of-smm-push-last
+    (implies (< (+ 1 (nfix n)) (len smm))
+             (equal (nth n new-smm) (nth n smm))))
+
+  (defret len-of-smm-push-last
+    (implies (not (equal 0 (len smm)))
+             (equal (len new-smm) (len smm)))))
+
+
+(define smm-check-truth-subcombs ((target-truth truth::truth4-p)
+                                  (other-truth truth::truth4-p)
+                                  (lit litp)
+                                  (idx natp)
+                                  (smm)
+                                  (eba))
+  :guard (and (< (+ 1 (lit-id lit)) (smm-nblocks smm))
+              (<= idx (smm-block-size (lit-id lit) smm))
+              (<= (ash 1 16) (eba-length eba)))
+  :measure (nfix (- (smm-block-size (lit-id lit) smm) (nfix idx)))
+  :returns (mv (target-found)
+               (new-smm)
+               (new-eba))
+  :prepwork ((local (defthm less-than-2^16-when-truth4-p
+                      (implies (and (truth::truth4-p x)
+                                    (<= 65536 y))
+                               (< x y))
+                      :hints(("Goal" :in-theory (enable truth::truth4-p)))))
+             (local (defthm not-greater-hack
+                      (implies (and (< x y)
+                                    (integerp x) (integerp y))
+                               (not (< y (+ 1 x)))))))
+  (b* ((block (lit-id lit))
+       ((when (mbe :logic (or (zp (- (smm-block-size block smm) (nfix idx)))
+                              (<= (smm-nblocks smm) (+ 1 (nfix block))))
+                   :exec (eql (smm-block-size block smm) idx)))
+        (mv nil smm eba))
+       (entry (smm-read block idx smm))
+       (conj (logand (truth::truth4-fix other-truth)
+                     (truth::truth-norm4 (logxor (- (lit-neg lit)) entry))))
+       ((when (eql conj (truth::truth4-fix target-truth)))
+        (mv t smm eba))
+       ((when (eql 1 (eba-get-bit conj eba)))
+        (smm-check-truth-subcombs target-truth other-truth lit (1+ (lnfix idx)) smm eba))
+       (eba (eba-set-bit conj eba))
+       (smm (smm-push-last conj smm)))
+    (smm-check-truth-subcombs target-truth other-truth lit (1+ (lnfix idx)) smm eba))
+  ///
+  (defret nth-of-smm-check-truth-subcombs
+    (implies (< (+ 1 (nfix n)) (len smm))
+             (equal (nth n new-smm) (nth n smm))))
+
+  (defret len-of-smm-check-truth-subcombs-smm
+    (implies (not (equal 0 (len smm)))
+             (equal (len new-smm) (len smm))))
+
+  (defret len-of-smm-check-truth-subcombs-eba
+    (implies (<= (ash 1 16) (len eba))
+             (equal (len new-eba)
+                    (len eba)))))
+
+
+(define smm-check-truth-subcombs-product ((target-truth truth::truth4-p)
+                                          (lit1 litp)
+                                          (lit2 litp)
+                                          (idx natp)
+                                          (smm)
+                                          (eba))
+  :guard (and (< (+ 1 (lit-id lit1)) (smm-nblocks smm))
+              (< (+ 1 (lit-id lit2)) (smm-nblocks smm))
+              (<= idx (smm-block-size (lit-id lit2) smm))
+              (<= (ash 1 16) (eba-length eba)))
+  :measure (nfix (- (smm-block-size (lit-id lit2) smm) (nfix idx)))
+  :returns (mv (target-found)
+               (new-smm)
+               (new-eba))
+  (b* (((when (mbe :logic (or (zp (- (smm-block-size (lit-id lit2) smm) (nfix idx)))
+                              (<= (smm-nblocks smm) (+ 1 (lit-id lit2))))
+                   :exec (eql idx (smm-block-size (lit-id lit2) smm))))
+        (mv nil smm eba))
+       (entry (smm-read (lit-id lit2) idx smm))
+       ((mv found smm eba)
+        (smm-check-truth-subcombs target-truth (truth::truth-norm4 entry)
+                                  lit1 0 smm eba))
+       ((when found) (mv found smm eba)))
+    (smm-check-truth-subcombs-product
+     target-truth lit1 lit2 (+ 1 (lnfix idx)) smm eba))
+  ///
+  (defret nth-of-smm-check-truth-subcombs-product
+    (implies (< (+ 1 (nfix n)) (len smm))
+             (equal (nth n new-smm) (nth n smm))))
+
+  (defret len-of-smm-check-truth-subcombs-product-smm
+    (implies (not (equal 0 (len smm)))
+             (equal (len new-smm) (len smm))))
+
+  (defret len-of-smm-check-truth-subcombs-product-eba
+    (implies (<= (ash 1 16) (len eba))
+             (equal (len new-eba)
+                    (len eba)))))
+
+(defstobj-clone eba2 eba :suffix "2")
+
+(define smm-push-aignet-cone-truths ((n natp)
+                                     (target-truth truth::truth4-p)
+                                     (eba "visited nodes")
+                                     (eba2 "existing truths")
+                                     (truth4arr)
+                                     (aignet)
+                                     (smm))
+  :guard (and (<= (nfix n) (max-fanin aignet))
+              (< (max-fanin aignet) (eba-length eba))
+              (< (max-fanin aignet) (truth4s-length truth4arr))
+              (equal (eba-length eba2) (ash 1 16))
+              (not (equal 0 (smm-nblocks smm))))
+  :returns (mv target-found new-eba new-eba2 new-smm)
+  :verify-guards nil
+  :prepwork ((local (defthm less-than-2^16-when-truth4-p
+                      (implies (and (truth::truth4-p x)
+                                    (<= 65536 y))
+                               (< x y))
+                      :hints(("Goal" :in-theory (enable truth::truth4-p)))))
+             (local (defthm not-greater-hack
+                      (implies (and (< x y)
+                                    (integerp x) (integerp y))
+                               (not (< y (+ 1 x))))))
+             (local (in-theory (disable lookup-id-out-of-bounds
+                                         acl2::nth-when-too-large-cheap))))
+  (b* (((when (eql (eba-get-bit n eba) 1)) (mv nil eba eba2 smm))
+       (eba (eba-set-bit n eba))
+       (type (id->type n aignet))
+       (truth (truth::get-truth4 n truth4arr))
+       (~truth (truth::truth-norm4 (lognot truth)))
+       ((when (or (eql (truth::truth4-fix target-truth) truth)
+                  (eql (truth::truth4-fix target-truth) ~truth)))
+        (mv t eba eba2 smm))
+       ((mv eba2 smm) (b* (((when (eql 1 (eba-get-bit truth eba2)))
+                            (mv eba2 smm))
+                           (eba2 (eba-set-bit truth eba2))
+                           (smm (smm-push-last truth smm)))
+                        (mv eba2 smm)))
+       ((mv eba2 smm) (b* (((when (eql 1 (eba-get-bit ~truth eba2)))
+                            (mv eba2 smm))
+                           (eba2 (eba-set-bit ~truth eba2))
+                           (smm (smm-push-last ~truth smm)))
+                        (mv eba2 smm))))
+    (aignet-case type
+      :out (smm-push-aignet-cone-truths (lit-id (co-id->fanin n aignet)) target-truth eba eba2 truth4arr aignet smm)
+      :gate (b* (((mv found eba eba2 smm)
+                  (smm-push-aignet-cone-truths (lit-id (gate-id->fanin0 n aignet)) target-truth eba eba2 truth4arr aignet smm))
+                 ((when found) (mv found eba eba2 smm)))
+              (smm-push-aignet-cone-truths (lit-id (gate-id->fanin1 n aignet)) target-truth eba eba2 truth4arr aignet smm))
+      :in (mv nil eba eba2 smm)
+      :const (mv nil eba eba2 smm)))
+  ///
+  (local (in-theory (disable (:d smm-push-aignet-cone-truths))))
+
+  (defret eba-len-of-smm-push-aignet-cone-truths
+    (implies (and (< (max-fanin aignet) (len eba))
+                  (<= (nfix n) (max-fanin aignet)))
+             (equal (len new-eba) (len eba)))
+    :hints (("goal" :expand (<call>) :induct <call>)))
+
+  (defret smm-len-of-smm-push-aignet-cone-truths
+    (implies (not (equal 0 (len smm)))
+             (equal (len new-smm) (len smm)))
+    :hints (("goal" :expand (<call>) :induct <call>)))
+
+  
+  (defret smm-nth-of-smm-push-aignet-cone-truths
+    (implies (< (+ 1 (nfix k)) (len smm))
+             (equal (nth k new-smm) (nth k smm)))
+    :hints (("goal" :expand (<call>) :induct <call>)))
+
+  (defret eba2-len-of-smm-push-aignet-cone-truths
+    (implies (<= (ash 1 16) (len eba2))
+             (equal (len new-eba2)
+                    (len eba2)))
+    :hints (("goal" :expand (<call>) :induct <call>)))
+
+  (verify-guards smm-push-aignet-cone-truths
+    :hints(("Goal" :in-theory (enable aignet-idp)))))
+
+
+
+(define maybe-grow-eba ((size natp) eba)
+  :returns (new-eba)
+  (if (< (lnfix size) (eba-length eba))
+      eba
+    (resize-eba (max 16 (* 2 (lnfix size))) eba))
+  ///
+  (defret len-of-maybe-grow-eba
+    (< (nfix size) (len new-eba))
+    :rule-classes :linear))
+
+(local
+ (encapsulate nil
+   (defthm lit-id-lte-max-fanin-of-aignet-and-gate-simp/strash-existing
+     (b* (((mv ?existing & ?nlit1 ?nlit2)
+           (aignet-and-gate-simp/strash lit1 lit2 gatesimp strash aignet)))
+       (implies (and (aignet-litp lit1 aignet)
+                     (aignet-litp lit2 aignet)
+                     existing)
+                (<= (lit-id existing) (node-count (find-max-fanin aignet)))))
+     :hints (("goal" :use aignet-litp-of-aignet-and-gate-simp/strash
+              :in-theory (disable aignet-litp-of-aignet-and-gate-simp/strash)))
+     :rule-classes (:rewrite :linear))
+
+   (defthm lit-id-lte-max-fanin-of-aignet-and-gate-simp/strash-nlit1
+     (b* (((mv ?existing & ?nlit1 ?nlit2)
+           (aignet-and-gate-simp/strash lit1 lit2 gatesimp strash aignet)))
+       (implies (and (aignet-litp lit1 aignet)
+                     (aignet-litp lit2 aignet))
+                (<= (lit-id nlit1) (node-count (find-max-fanin aignet)))))
+     :hints (("goal" :use aignet-litp-of-aignet-and-gate-simp/strash
+              :in-theory (disable aignet-litp-of-aignet-and-gate-simp/strash)))
+     :rule-classes (:rewrite :linear))
+
+   (defthm lit-id-lte-max-fanin-of-aignet-and-gate-simp/strash-nlit2
+     (b* (((mv ?existing & ?nlit1 ?nlit2)
+           (aignet-and-gate-simp/strash lit1 lit2 gatesimp strash aignet)))
+       (implies (and (aignet-litp lit1 aignet)
+                     (aignet-litp lit2 aignet))
+                (<= (lit-id nlit2) (node-count (find-max-fanin aignet)))))
+     :hints (("goal" :use aignet-litp-of-aignet-and-gate-simp/strash
+              :in-theory (disable aignet-litp-of-aignet-and-gate-simp/strash)))
+     :rule-classes (:rewrite :linear))))
+
+(def-statsmgr libstats
+  (product)
+  (top-and)
+  (subnode)
+  (over-count)
+  (existing)
+
+(defstobj libstats
+  (libstats-product :type (integer 0 *) :initially 0)
+  (libstats-top-and :type (integer 0 *) :initially 0)
+  (libstats-subnode :type (integer 0 *) :initially 0)
+  (libstats-over-count :type (integer 0 *) :initially 0)
+  (libstats-existing :type (integer 0 *) :initially 0))
+
+(define libstats-init (libstats)
+  (b* ((libstats (update-libstats-product 0 libstats))
+       (libstats (update-libstats-top-and 0 libstats))
+       (libstats (update-libstats-subnode 0 libstats))
+       (libstats (update-libstats-over-count 0 libstats))
+       (libstats (update-libstats-existing 0 libstats)))
+    libstats))
+
+(define incr-libstats-product (libstats)
+  (update-libstats-product (+ 1 (libstats-product libstats)) libstats))
+
+(define incr-libstats-top-and (libstats)
+  (update-libstats-top-and (+ 1 (libstats-top-and libstats)) libstats))
+
+(define incr-libstats-subnode (libstats)
+  (update-libstats-subnode (+ 1 (libstats-subnode libstats)) libstats))
+
+(define incr-libstats-over-count (libstats)
+  (update-libstats-over-count (+ 1 (libstats-over-count libstats)) libstats))
+
+(define incr-libstats-existing (libstats)
+  (update-libstats-existing (+ 1 (libstats-existing libstats)) libstats))
+
+(define print-libstats (libstats)
+  (progn$ (cw "product: ~x0~%" (libstats-product libstats))
+          (cw "top-and: ~x0~%" (libstats-top-and libstats))
+          (cw "subnode: ~x0~%" (libstats-subnode libstats))
+          (cw "over-count: ~x0~%" (libstats-over-count libstats))
+          (cw "existing: ~x0~%" (libstats-existing libstats))))
+
+(define aignet-and-if-not-redundant ((nlit litp)
+                                     (mlit litp)
+                                     (eba)
+                                     (eba2)
+                                     (truth4arr)
+                                     (smm)
+                                     (strash)
+                                     (aignet)
+                                     (libstats)
+                                     (lits-acc lit-listp))
+  :returns (mv (new-lits-acc lit-listp)
+               (new-eba)
+               (new-eba2)
+               (new-truth4arr)
+               (new-smm)
+               (new-strash)
+               (new-aignet)
+               (new-libstats))
+  :guard (and (fanin-litp nlit aignet)
+              (fanin-litp mlit aignet)
+              (equal (num-outs aignet) 0)
+              (equal (num-nxsts aignet) 0)
+              (< (max-fanin aignet) (eba-length eba))
+              (equal (eba-length eba2) (ash 1 16))
+              (< (max-fanin aignet) (truth4s-length truth4arr))
+              (equal (smm-nblocks smm) (+ 1 (num-nodes aignet))))
+  :guard-debug t
+  :prepwork ((local (in-theory (disable aignet-install-and-of-aignet-and-gate-simp/strash
+                                        (acl2::repeat) len)))
+             (local (in-theory (enable aignet-install-and)))
+             (local (defthm lte-max-fanin-when-aignet-litp
+                      (implies (aignet-litp lit aignet)
+                               (<= (lit-id lit) (node-count (find-max-fanin aignet))))
+                      :hints(("Goal" :in-theory (enable aignet-litp))))))
+  (b* (((mv existing key lit1 lit2) (aignet-and-gate-simp/strash nlit mlit
+                                                                 9 strash aignet))
+       ((when existing)
+        (b* ((libstats (incr-libstats-existing libstats)))
+          (mv (lit-list-fix lits-acc)
+              eba eba2 truth4arr smm strash aignet libstats)))
+       (eba (eba-clear eba))
+       ((mv count1 eba) (aignet-count-gates-eba (lit-id lit1) eba aignet))
+       ((mv count2 eba) (aignet-count-gates-eba (lit-id lit2) eba aignet))
+       (count (+ 1 count1 count2))
+       ((when (< 7 count))
+        (b* ((libstats (incr-libstats-over-count libstats)))
+          (mv (lit-list-fix lits-acc)
+              eba eba2 truth4arr smm strash aignet libstats)))
+       (truth1 (truth::lit-truth lit1 truth4arr))
+       (truth2 (truth::lit-truth lit2 truth4arr))
+       (and-truth (logand truth1 truth2))
+       (smm (smm-resize-last 0 smm))
+       (eba2 (eba-clear eba2))
+       ;; (smm (smm-resize-last 0 smm))
+       ;; (eba2 (eba-clear eba2))
+       (eba (eba-clear eba))
+       ((mv target-found eba eba2 smm) (smm-push-aignet-cone-truths (lit-id lit1) and-truth eba eba2 truth4arr aignet smm))
+       ((when target-found)
+        (b* ((libstats (incr-libstats-subnode libstats)))
+          (mv (lit-list-fix lits-acc)
+              eba eba2 truth4arr smm strash aignet libstats)))
+       ((mv target-found eba eba2 smm) (smm-push-aignet-cone-truths (lit-id lit2) and-truth eba eba2 truth4arr aignet smm))
+       ((when target-found)
+        (b* ((libstats (incr-libstats-subnode libstats)))
+          (mv (lit-list-fix lits-acc)
+              eba eba2 truth4arr smm strash aignet libstats)))
+       ((mv target-found smm eba2)
+        (smm-check-truth-subcombs and-truth truth1 lit2 0 smm eba2))
+       ((when target-found)
+        (b* ((libstats (incr-libstats-top-and libstats)))
+          (mv (lit-list-fix lits-acc)
+              eba eba2 truth4arr smm strash aignet libstats)))
+       ((mv target-found smm eba2)
+        (smm-check-truth-subcombs and-truth truth2 lit1 0 smm eba2))
+       ((when target-found)
+        (b* ((libstats (incr-libstats-top-and libstats)))
+          (mv (lit-list-fix lits-acc)
+              eba eba2 truth4arr smm strash aignet libstats)))
+       ((mv target-found smm eba2)
+        (smm-check-truth-subcombs-product and-truth lit1 lit2 0 smm eba2))
+       ((when target-found)
+        (b* ((libstats (incr-libstats-product libstats)))
+          (mv (lit-list-fix lits-acc)
+              eba eba2 truth4arr smm strash aignet libstats)))
+       ;; We want the last element of smm to contain all truth tables that can
+       ;; be achieved by replacing some subtree of n with some subtree of that
+       ;; subtree.  I think the worst case for this in 7 gates is a linear tree
+       ;; 7 nodes deep (with 8 leaves).  The top node can be replaced by any of
+       ;; its subnodes or their negations: 6 gates + 8 leaves * 2, the
+       ;; next-highest can be replaced by any of its -- 5 gates + 7 leaves * 2,
+       ;; etc., so total is (14 + 12 + 10 + 8 + 6 + 4 + 2) * 2 = 112 -- not too
+       ;; bad.  Do we need to allow replacement of subtrees with constants?  I
+       ;; think not, because these bubble up and reduce to replacing some
+       ;; higher subtree with its other subtree, which we've already allowed.
+
+       ;; The last element of smm now contains all the truth tables that can be
+       ;; obtained by ANDing n with the result of replacing any subtree of m
+       ;; with a subtree of that subtree, and vice versa.  That is, those truth
+       ;; tables that can be obtained by replacing a subtree of n or m by one
+       ;; of their subtrees.  It remains to include the results of replacing
+       ;; the top node with one of its subtrees, i.e., all the truth tables of
+       ;; the subnodes themselves.
+
+       (new-id (num-nodes aignet))
+       ((mv lit strash aignet) (aignet-install-and nil key lit1 lit2 strash aignet))
+       (truth4arr (truth::maybe-grow-truth4arr new-id truth4arr))
+       (truth4arr (truth::set-truth4 new-id and-truth truth4arr))
+       (eba (maybe-grow-eba new-id eba))
+       (smm (smm-addblock 0 smm)))
+    (mv (cons lit (lit-list-fix lits-acc))
+        eba eba2 truth4arr smm strash aignet libstats))
+  ///
+  
+
+  (def-aignet-preservation-thms aignet-and-if-not-redundant :stobjname aignet)
+
+  (defret aignet-litp-of-aignet-and-if-not-redundant
+    (implies (and (aignet-litp nlit aignet)
+                  (aignet-litp mlit aignet)
+                  (aignet-lit-listp lits-acc aignet))
+             (aignet-lit-listp new-lits-acc new-aignet)))
+
+  ;; (defret aignet-and-if-not-redundant-correct
+  ;;   (implies (and (aignet-litp nlit aignet)
+  ;;                 (aignet-litp mlit aignet)
+  ;;                 new-lit)
+  ;;            (equal (lit-eval new-lit invals regvals new-aignet)
+  ;;                   (eval-and-of-lits nlit mlit invals regvals aignet)))
+  ;;   :hints(("Goal" :expand ((:free (n aignet)
+  ;;                            (lit-eval (make-lit n 0) invals regvals aignet))))))
+
+  (defret truth4arr-length-of-aignet-and-if-not-redundant
+    (implies (< (node-count (find-max-fanin aignet)) (len truth4arr))
+             (< (node-count (find-max-fanin new-aignet)) (len new-truth4arr)))
+    :rule-classes (:rewrite (:linear :trigger-terms ((len new-truth4arr)))))
+
+  (defret eba-length-of-aignet-and-if-not-redundant
+    (implies (and (< (node-count (find-max-fanin aignet)) (len eba))
+                  (aignet-litp nlit aignet)
+                  (aignet-litp mlit aignet))
+             (< (node-count (find-max-fanin new-aignet)) (len new-eba)))
+    :rule-classes (:rewrite (:linear :trigger-terms ((len new-eba)))))
+
+  (defret eba2-length-of-aignet-and-if-not-redundant
+    (implies (<= (ash 1 16) (len eba2))
+             (equal (len new-eba2) (len eba2))))
+
+  (defret smm-nblocks-of-aignet-and-if-not-redundant
+    (implies (equal (len smm) (+ 1 (num-nodes aignet)))
+             (equal (len new-smm) (+ 1 (num-nodes new-aignet)))))
+
+  (defret stype-count-of-aignet-and-if-not-redundant
+    (implies (not (equal (stype-fix stype) :gate))
+             (equal (stype-count stype new-aignet)
+                    (stype-count stype aignet))))
+
+  ;; (defret max-fanin-of-aignet-and-if-not-redundant
+  ;;   (implies (equal (node-count (find-max-fanin aignet)) (node-count aignet))
+  ;;            (equal (find-max-fanin new-aignet)
+  ;;                   (node-list-fix new-aignet))))
+  )
+
+
+
+       
+
+(define aignet-ands-if-not-redundant ((n litp)
+                                      (m litp)
+                                      (eba "bit array marked with n's cone")
+                                      (eba2 "bit array to be marked with m's cone")
+                                      (truth4arr "truth values of aignet ids")
+                                      (smm)
+                                      (strash)
+                                      (aignet)
+                                      (libstats)
+                                      (lits-acc lit-listp))
+  :guard (and (fanin-litp n aignet)
+              (fanin-litp m aignet)
+              (equal (num-outs aignet) 0)
+              (equal (num-nxsts aignet) 0)
+              (< (max-fanin aignet) (eba-length eba))
+              (equal (eba-length eba2) (ash 1 16))
+              (< (max-fanin aignet) (truth4s-length truth4arr))
+              (equal (smm-nblocks smm) (+ 1 (num-nodes aignet))))
+  :guard-hints (("goal" :do-not-induct t))
+  :returns (mv (new-lits-acc lit-listp)
+               (new-eba)
+               (new-eba2)
+               (new-truth4arr)
+               (new-smm)
+               (new-strash)
+               (new-aignet)
+               (new-libstats))
+  :prepwork ((local (in-theory (disable len acl2::repeat-when-zp aignet-lit-listp
+                                        SATLINK::EQUAL-OF-LIT-NEGATE-COND-COMPONENT-REWRITES
+                                        FANIN-IF-CO-ID-LTE-MAX-FANIN
+                                        NODE-COUNT-OF-FIND-MAX-FANIN-OF-EXTENSION))))
+  (b* ((~n (lit-negate n))
+       (~m (lit-negate m))
+       ((mv lits-acc eba eba2 truth4arr smm strash aignet libstats)
+        (aignet-and-if-not-redundant n m eba eba2 truth4arr smm strash aignet libstats lits-acc))
+       ((mv lits-acc eba eba2 truth4arr smm strash aignet libstats)
+        (aignet-and-if-not-redundant n ~m eba eba2 truth4arr smm strash aignet libstats lits-acc))
+       ((mv lits-acc eba eba2 truth4arr smm strash aignet libstats)
+        (aignet-and-if-not-redundant ~n m eba eba2 truth4arr smm strash aignet libstats lits-acc)))
+    (aignet-and-if-not-redundant ~n ~m eba eba2 truth4arr smm strash aignet libstats lits-acc))
+  ///
+
+  ;; (local (in-theory (disable max-fanin-of-aignet-and-if-not-redundant)))
+  
+  (def-aignet-preservation-thms aignet-ands-if-not-redundant :stobjname aignet)
+
+  (defret aignet-litp-of-aignet-ands-if-not-redundant
+    (implies (and (aignet-litp n aignet)
+                  (aignet-litp m aignet)
+                  (aignet-lit-listp lits-acc aignet))
+             (aignet-lit-listp new-lits-acc new-aignet)))
+
+  ;; (defret aignet-truthmap-p-of-aignet-ands-if-not-redundant
+  ;;   (implies (aignet-truthmap-p truthmap aignet)
+  ;;            (aignet-truthmap-p new-truthmap new-aignet))
+  ;;   :hints (("goal" :expand ((:free (a b aignet) (aignet-truthmap-p (cons a b) aignet))))))
+
+  (defret truth4arr-length-of-aignet-ands-if-not-redundant
+    (implies (< (node-count (find-max-fanin aignet)) (len truth4arr))
+             (< (node-count (find-max-fanin new-aignet)) (len new-truth4arr)))
+    :rule-classes :linear)
+
+  (defret eba-length-of-aignet-ands-if-not-redundant
+    (implies (and (< (node-count (find-max-fanin aignet)) (len eba))
+                  (aignet-litp n aignet)
+                  (aignet-litp m aignet))
+             (< (node-count (find-max-fanin new-aignet)) (len new-eba)))
+    :rule-classes :linear)
+
+  (defret eba2-length-of-aignet-ands-if-not-redundant
+    (implies (<= (ash 1 16) (len eba2))
+             (equal (len new-eba2) (len eba2))))
+
+  (defret stype-count-of-aignet-ands-if-not-redundant
+    (implies (not (equal (stype-fix stype) :gate))
+             (equal (stype-count stype new-aignet)
+                    (stype-count stype aignet))))
+
+
+  (defret smm-nblocks-of-aignet-ands-if-not-redundant
+    (implies (equal (len smm) (+ 1 (num-nodes aignet)))
+             (equal (len new-smm) (+ 1 (num-nodes new-aignet)))))
+
+  ;; (local (in-theory (enable max-fanin-of-aignet-and-if-not-redundant)))
+
+  ;; (defret max-fanin-of-aignet-ands-if-not-redundant
+  ;;   (implies (equal (node-count (find-max-fanin aignet)) (node-count aignet))
+  ;;            (equal (find-max-fanin new-aignet)
+  ;;                   (node-list-fix new-aignet))))
+  )
+
+
+(local (defthm stype-when-stype-count-0
+         (implies (and (aignet-extension-bind-inverse)
+                       (equal (stype-count stype new) 0)
+                       (not (equal (stype-fix stype) :const)))
+                  (not (equal (stype (car orig)) stype)))
+         :hints(("Goal" :in-theory (enable aignet-extension-p stype-count)))))
+
+
+(local (defthm aignet-litp-when-no-outs
+         (implies (and (equal (stype-count :po aignet) 0)
+                       (equal (stype-count :nxst aignet) 0))
+                  (equal (aignet-litp lit aignet)
+                         (< (lit-id lit) (num-nodes aignet))))
+         :hints(("Goal" :in-theory (enable aignet-litp ctype)
+                 :cases ((< (lit-id lit) (num-nodes aignet)))))))
+
+
+(define aignet-and-lits-with-node ((lit litp)
+                                   (lits lit-listp)
+                                   (eba "bit array marked with lit's cone")
+                                   (eba2 "bit array to be marked with lits' cone")
+                                   (truth4arr "truth values of aignet ids")
+                                   (smm)
+                                   (strash)
+                                   (aignet)
+                                   (libstats)
+                                   (lits-acc lit-listp))
+  :guard (and (aignet-lit-listp lits aignet)
+              (fanin-litp lit aignet)
+              (equal (num-outs aignet) 0)
+              (equal (num-nxsts aignet) 0)
+              (< (max-fanin aignet) (eba-length eba))
+              (eql (eba-length eba2) (ash 1 16))
+              (< (max-fanin aignet) (truth4s-length truth4arr))
+              (equal (smm-nblocks smm) (+ 1 (num-nodes aignet))))
+  :guard-hints (("goal" :do-not-induct t))
+  :returns (mv (new-lits-acc lit-listp)
+               (new-eba)
+               (new-eba2)
+               (new-truth4arr)
+               (new-smm)
+               (new-strash)
+               (new-aignet)
+               (new-libstats))
+  :measure (len lits)
+  (b* (((when (atom lits))
+        (mv (lit-list-fix lits-acc)
+            eba eba2 truth4arr smm strash aignet libstats))
+       ((mv lits-acc eba eba2 truth4arr smm strash aignet libstats)
+        (aignet-ands-if-not-redundant
+         lit (car lits) eba eba2 truth4arr smm strash aignet libstats lits-acc)))
+    (aignet-and-lits-with-node lit (cdr lits) eba eba2 truth4arr smm strash aignet libstats lits-acc))
+  ///
+
+  
+  
+  (def-aignet-preservation-thms aignet-and-lits-with-node :stobjname aignet)
+
+  (defret aignet-litp-of-aignet-and-lits-with-node
+    (implies (and (aignet-litp lit aignet)
+                  (aignet-lit-listp lits aignet)
+                  (aignet-lit-listp lits-acc aignet))
+             (aignet-lit-listp new-lits-acc new-aignet))
+    :hints (("goal" :induct <call> :expand (<call>))))
+
+  ;; (defret aignet-truthmap-p-of-aignet-and-lits-with-node
+  ;;   (implies (aignet-truthmap-p truthmap aignet)
+  ;;            (aignet-truthmap-p new-truthmap new-aignet))
+  ;;   :hints (("goal" :expand ((:free (a b aignet) (aignet-truthmap-p (cons a b) aignet))))))
+
+  (defret truth4arr-length-of-aignet-and-lits-with-node
+    (implies (< (node-count (find-max-fanin aignet)) (len truth4arr))
+             (< (node-count (find-max-fanin new-aignet)) (len new-truth4arr)))
+    :rule-classes (:rewrite (:linear :trigger-terms ((node-count (find-max-fanin new-aignet))
+                                                     (len new-truth4arr)))))
+
+  (defret eba-length-of-aignet-and-lits-with-node
+    (implies (and (< (node-count (find-max-fanin aignet)) (len eba))
+                  (aignet-litp lit aignet)
+                  (aignet-lit-listp lits aignet))
+             (< (node-count (find-max-fanin new-aignet)) (len new-eba)))
+    :hints (("goal" :induct <call> :expand (<call>)))
+    :rule-classes (:rewrite (:linear :trigger-terms ((node-count (find-max-fanin new-aignet))
+                                                     (len new-eba)))))
+
+  (defret eba2-length-of-aignet-and-lits-with-node
+    (implies (<= (ash 1 16) (len eba2))
+             (equal (len new-eba2) (len eba2)))
+    :hints (("goal" :induct <call> :expand (<call>))))
+
+  (defret stype-count-of-aignet-and-lits-with-node
+    (implies (not (equal (stype-fix stype) :gate))
+             (equal (stype-count stype new-aignet)
+                    (stype-count stype aignet))))
+
+  (defret smm-nblocks-of-aignet-and-lits-with-node
+    (implies (equal (len smm) (+ 1 (num-nodes aignet)))
+             (equal (len new-smm) (+ 1 (num-nodes new-aignet))))))
+
+(local (defthmd max-fanin-when-no-outs
+         (implies (and (equal (stype-count :po aignet) 0)
+                       (equal (stype-count :nxst aignet) 0))
+                  (equal (find-max-fanin aignet)
+                         (node-list-fix aignet)))
+         :hints(("Goal" :in-theory (enable find-max-fanin ctype)
+                 :expand ((find-max-fanin aignet))
+                 :do-not-induct t))))
+
+(define aignet-and-lits-with-nodes-up-to ((m posp)
+                                          (max-m posp)
+                                          (lits lit-listp)
+                                          (eba "bit array marked with n's cone")
+                                          (eba2 "bit array to be marked with m's cone")
+                                          (truth4arr "truth values of aignet ids")
+                                          (smm)
+                                          (strash)
+                                          (aignet)
+                                          (libstats)
+                                          (lits-acc lit-listp))
+  :guard (and (equal (num-outs aignet) 0)
+              (equal (num-nxsts aignet) 0)
+              (aignet-lit-listp lits aignet)
+              (<= max-m (num-nodes aignet))
+              (<= m max-m)
+              (< (max-fanin aignet) (eba-length eba))
+              (eql (eba-length eba2) (ash 1 16))
+              (< (max-fanin aignet) (truth4s-length truth4arr))
+              (equal (smm-nblocks smm) (+ 1 (num-nodes aignet))))
+  :guard-debug t
+  :guard-hints (("goal" :do-not-induct t))
+  :returns (mv (new-lits-acc lit-listp)
+               (new-eba)
+               (new-eba2)
+               (new-truth4arr)
+               (new-smm)
+               (new-strash)
+               (new-aignet)
+               (new-libstats))
+  ;; :guard-debug t
+  :measure (nfix (- (lposfix max-m) (lposfix m)))
+  (b* (((when (mbe :logic (zp (- (lposfix max-m) (lposfix m)))
+                   :exec (eql m max-m)))
+        (mv (lit-list-fix lits-acc)
+            eba eba2 truth4arr smm strash aignet libstats))
+       (m (lposfix m))
+       (lit (mk-lit m 0))
+       ((mv lits-acc eba eba2 truth4arr smm strash aignet libstats)
+        (aignet-and-lits-with-node
+         lit lits eba eba2 truth4arr smm strash aignet libstats lits-acc)))
+    (aignet-and-lits-with-nodes-up-to (1+ (lposfix m)) max-m lits eba eba2 truth4arr smm strash aignet libstats lits-acc))
+  ///
+
+  
+  
+  (def-aignet-preservation-thms aignet-and-lits-with-nodes-up-to :stobjname aignet)
+
+  (defret aignet-litp-of-aignet-and-lits-with-nodes-up-to
+    (implies (and (aignet-lit-listp lits aignet)
+                  (equal (stype-count :po aignet) 0)
+                  (equal (stype-count :nxst aignet) 0)
+                  (<= (lposfix max-m) (+ 1 (node-count aignet)))
+                  (aignet-lit-listp lits-acc aignet))
+             (aignet-lit-listp new-lits-acc new-aignet)))
+
+  ;; (defret aignet-truthmap-p-of-aignet-and-lits-with-nodes-up-to
+  ;;   (implies (aignet-truthmap-p truthmap aignet)
+  ;;            (aignet-truthmap-p new-truthmap new-aignet))
+  ;;   :hints (("goal" :expand ((:free (a b aignet) (aignet-truthmap-p (cons a b) aignet))))))
+
+  (defret truth4arr-length-of-aignet-and-lits-with-nodes-up-to
+    (implies (< (node-count (find-max-fanin aignet)) (len truth4arr))
+             (< (node-count (find-max-fanin new-aignet)) (len new-truth4arr)))
+    :rule-classes (:rewrite (:linear :trigger-terms ((node-count (find-max-fanin new-aignet))
+                                                     (len new-truth4arr)))))
+
+  (local (defthm <=-max-fanin-when-<=-node-count
+           (implies (and (equal (stype-count :po aignet) 0)
+                         (equal (stype-count :nxst aignet) 0)
+                         (< n (+ 1 (node-count aignet)))
+                         (natp n))
+                    (<= n (node-count (find-max-fanin aignet))))
+           :hints(("Goal" :in-theory (enable max-fanin-when-no-outs)))))
+
+  (defret eba-length-of-aignet-and-lits-with-nodes-up-to
+    (implies (and (aignet-lit-listp lits aignet)
+                  (equal (stype-count :po aignet) 0)
+                  (equal (stype-count :nxst aignet) 0)
+                  (<= (lposfix max-m) (+ 1 (node-count aignet)))o
+                  (< (node-count (find-max-fanin aignet)) (len eba)))
+             (< (node-count (find-max-fanin new-aignet)) (len new-eba)))
+    :hints (("Goal" :induct <call> :expand (<call>)))
+    :rule-classes (:rewrite (:linear :trigger-terms ((node-count (find-max-fanin new-aignet))
+                                                     (len new-eba)))))
+
+  (defret eba2-length-of-aignet-and-lits-with-nodes-up-to
+    (implies (<= (ash 1 16) (len eba2))
+             (equal (len new-eba2) (len eba2))))
+
+  (defret stype-count-of-aignet-and-lits-with-nodes-up-to
+    (implies (not (equal (stype-fix stype) :gate))
+             (equal (stype-count stype new-aignet)
+                    (stype-count stype aignet))))
+
+  (defret smm-nblocks-of-aignet-and-lits-with-nodes-up-to
+    (implies (equal (len smm) (+ 1 (num-nodes aignet)))
+             (equal (len new-smm) (+ 1 (num-nodes new-aignet))))))
+
+
+(define aignet-make-lit-products ((curr-level natp)
+                                  (max-level natp)
+                                  (prev-lits lit-listp)
+                                  (eba "bit array marked with n's cone")
+                                  (eba2 "bit array to be marked with m's cone")
+                                  (truth4arr "truth values of aignet ids")
+                                  (smm)
+                                  (strash)
+                                  (aignet)
+                                  (libstats))
+  :guard (and (equal (num-outs aignet) 0)
+              (equal (num-nxsts aignet) 0)
+              (aignet-lit-listp prev-lits aignet)
+              (<= curr-level max-level)
+              (< (max-fanin aignet) (eba-length eba))
+              (eql (ash 1 16) (eba-length eba2))
+              (< (max-fanin aignet) (truth4s-length truth4arr))
+              (eql (smm-nblocks smm) (+ 1 (num-nodes aignet))))
+  :guard-hints (("goal" :do-not-induct t :expand ((aignet-lit-listp lits aignet)))
+                (and stable-under-simplificationp
+                     '(:in-theory (enable max-fanin-when-no-outs))))
+  ;; :guard-debug t
+  :returns (mv ;; (new-lits lit-listp)
+               (new-eba)
+               (new-eba2)
+               (new-truth4arr)
+               (new-smm)
+               (new-strash)
+               (new-aignet)
+               (new-libstats))
+  :measure (nfix (- (nfix max-level) (nfix curr-level)))
+  (b* ((- (cw "Level ~x0: ~x1 new lits, ~x2 nodes total~%" curr-level
+              (len prev-lits) (num-nodes aignet)))
+       (- (print-libstats libstats))
+       ((when (mbe :logic (zp (- (nfix max-level) (nfix curr-level)))
+                   :exec (eql max-level curr-level)))
+        (mv eba eba2 truth4arr smm strash aignet libstats))
+       (curr-nodes (num-nodes aignet))
+       ((mv next-lits eba eba2 truth4arr smm strash aignet libstats)
+        (aignet-and-lits-with-nodes-up-to 1 curr-nodes prev-lits eba eba2 truth4arr smm strash aignet libstats nil)))
+    (aignet-make-lit-products (1+ (lnfix curr-level)) max-level next-lits eba eba2 truth4arr smm strash aignet libstats))
+  ///
+
+    
+  (def-aignet-preservation-thms aignet-make-lit-products :stobjname aignet)
+
+  ;; (defret aignet-truthmap-p-of-aignet-make-lit-products
+  ;;   (implies (aignet-truthmap-p truthmap aignet)
+  ;;            (aignet-truthmap-p new-truthmap new-aignet))
+  ;;   :hints (("goal" :expand ((:free (a b aignet) (aignet-truthmap-p (cons a b) aignet))))))
+
+  (defret truth4arr-length-of-aignet-make-lit-products
+    (implies (< (node-count (find-max-fanin aignet)) (len truth4arr))
+             (< (node-count (find-max-fanin new-aignet)) (len new-truth4arr)))
+    :rule-classes :linear)
+
+  (defret eba-length-of-aignet-make-lit-products
+    (implies (and (aignet-lit-listp prev-lits aignet)
+                  (equal (stype-count :po aignet) 0)
+                  (equal (stype-count :nxst aignet) 0)
+                  (< (node-count (find-max-fanin aignet)) (len eba)))
+             (< (node-count (find-max-fanin new-aignet)) (len new-eba)))
+    :hints (("Goal" :induct <call> :expand (<call>)))
+    :rule-classes :linear)
+
+  (defret eba2-length-of-aignet-make-lit-products
+    (implies (<= (expt 2 16) (len eba2))
+             (equal (len new-eba2) (len eba2))))
+
+  (defret stype-count-of-aignet-make-lit-products
+    (implies (not (equal (stype-fix stype) :gate))
+             (equal (stype-count stype new-aignet)
+                    (stype-count stype aignet))))
+
+  (defret smm-nblocks-of-aignet-make-lit-products
+    (implies (equal (len smm) (+ 1 (num-nodes aignet)))
+             (equal (len new-smm) (+ 1 (num-nodes new-aignet))))))
+    
+       
+(define aignet-make-levels-aux ((max-levels natp)
+                                (truth4arr)
+                                (aignet)
+                                (smm)
+                                (eba)
+                                (eba2)
+                                (strash)
+                                (libstats))
+  :prepwork ((local (include-book "std/lists/resize-list" :dir :System))
+             (local (in-theory (disable (resize-eba) (resize-truth4s) (resize-list) (acl2::repeat)))))
+  :returns (mv new-eba new-eba2 new-truth4arr new-smm new-strash new-aignet new-libstats)
+  (b* ((smm (smm-clear smm))
+       (eba (resize-eba 0 eba))
+       (eba2 (resize-eba2 0 eba2))
+       (strash (strashtab-clear strash))
+       (aignet (aignet-init 0 0 4 50000 aignet))
+       (truth4arr (resize-truth4s 1000 truth4arr))
+       (aignet (aignet-add-in aignet))
+       (aignet (aignet-add-in aignet))
+       (aignet (aignet-add-in aignet))
+       (aignet (aignet-add-in aignet))
+       (start-lits '(2 4 6 8)) ;; input lits
+       (truth4arr (truth::set-truth4 0 0 truth4arr))
+       (truth4arr (truth::set-truth4 1 (truth::var4 0) truth4arr))
+       (truth4arr (truth::set-truth4 2 (truth::var4 1) truth4arr))
+       (truth4arr (truth::set-truth4 3 (truth::var4 2) truth4arr))
+       (truth4arr (truth::set-truth4 4 (truth::var4 3) truth4arr))
+       (smm (smm-addblock 0 smm))
+       (smm (smm-addblock 0 smm))
+       (smm (smm-addblock 0 smm))
+       (smm (smm-addblock 0 smm))
+       (smm (smm-addblock 0 smm))
+       (smm (smm-addblock 0 smm))
+       (eba (resize-eba 1000 eba))
+       (eba2 (resize-eba (ash 1 16) eba2))
+       (libstats (libstats-init libstats)))
+    (aignet-make-lit-products 0 max-levels start-lits eba eba2 truth4arr smm strash aignet libstats))
+  ///
+  
+  (defret truth4arr-length-of-aignet-make-levels-aux
+    (< (node-count (find-max-fanin new-aignet)) (len new-truth4arr))
+    :rule-classes :linear)
+
+  (defret stype-count-of-aignet-make-levels-aux
+    (and (equal (stype-count :pi new-aignet) 4)
+         (equal (stype-count :reg new-aignet) 0)
+         (equal (stype-count :po new-aignet) 0)
+         (equal (stype-count :nxst new-aignet) 0))))
+  
+
+
+(define aignet-make-levels ((max-levels natp)
+                            (truth4arr)
+                            (aignet))
+  :returns (mv ;; (new-truthmap truthmap-p)
+               (new-truth4arr)
+               (new-aignet))
+  (b* (((acl2::local-stobjs eba eba2 smm strash libstats)
+        (mv eba eba2 truth4arr smm strash aignet libstats)))
+    (aignet-make-levels-aux max-levels truth4arr aignet smm eba eba2 strash libstats))
+  ///
+  
+  ;; (defret aignet-truthmap-p-of-aignet-make-levels
+  ;;   (aignet-truthmap-p new-truthmap new-aignet)
+  ;;   :hints (("goal" :expand ((:free (a b aignet) (aignet-truthmap-p (cons a b) aignet))))))
+
+  (defret truth4arr-length-of-aignet-make-levels
+    (< (node-count (find-max-fanin new-aignet)) (len new-truth4arr))
+    :rule-classes :linear)
+
+  (defret stype-count-of-aignet-make-levels
+    (and (equal (stype-count :pi new-aignet) 4)
+         (equal (stype-count :reg new-aignet) 0)
+         (equal (stype-count :po new-aignet) 0)
+         (equal (stype-count :nxst new-aignet) 0))))
+       
+                                     
+
+
+
+(include-book "std/util/defconsts" :dir :system)
+
+(defconsts (truth4arr aignet) (aignet-make-levels 3 truth4arr aignet))
+(defconsts (truth4arr aignet) (aignet-make-levels 4 truth4arr aignet))
+(defconsts (eba eba2 truth4arr smm strash aignet libstats) (aignet-make-levels-aux 4 truth4arr aignet smm eba eba2 strash libstats))
+
+
+
+
+
+
+
+
+
+
+
+
+
+
+
+(fty::defmap truthmap :key-type truth4 :val-type lit-listp)
+
+(define aignet-truthmap-p ((x truthmap-p) aignet)
+  (if (atom x)
+      t
+    (if (mbt (and (consp (car x))
+                  (truth4-p (caar x))))
+        (and (aignet-lit-listp (cdar x) aignet)
+             (aignet-truthmap-p (cdr x) aignet))
+      (aignet-truthmap-p (cdr x) aignet)))
+  ///
+  (defthm aignet-lit-listp-of-aignet-truthmap-lookup
+    (implies (and (aignet-truthmap-p x aignet)
+                  (truth4-p k))
+             (aignet-lit-listp (cdr (hons-assoc-equal k x)) aignet))
+    :hints(("Goal" :in-theory (enable hons-assoc-equal))))
+
+  (local (defthm truthmap-fix-when-first-bad
+           (implies (and (consp x)
+                         (not (and (consp (car x))
+                                   (truth4-p (caar x)))))
+                    (equal (truthmap-fix x)
+                           (truthmap-fix (cdr x))))
+           :hints(("Goal" :in-theory (enable truthmap-fix)))))
+
+  (defthm aignet-truthmap-p-of-extension
+    (implies (and (aignet-extension-binding)
+                  (aignet-truthmap-p x orig))
+             (aignet-truthmap-p x new)))
+
+  (local (in-theory (disable (:d aignet-truthmap-p)))))
+
+
+
+
+(define lit-has-marked-children ((x litp)
+                                 (eba)
+                                 (eba2)
+                                 (aignet))
+  :guard (and (fanin-litp x aignet)
+              (< (max-fanin aignet) (eba-length eba))
+              (< (max-fanin aignet) (eba-length eba2)))
+  (b* ((n (lit-id x))
+       ((when (or (eql n 0)
+                  (eql 1 (eba-get-bit n eba))
+                  (eql 1 (eba-get-bit n eba2))))
+        t)
+       (type (id->type n aignet)))
+    (aignet-case type
+      :gate (b* ((child0 (lit-id (gate-id->fanin0 n aignet)))
+                 (child1 (lit-id (gate-id->fanin1 n aignet))))
+              (and (or (not (eql (id->type child0 aignet) (gate-type)))
+                       (eql 1 (eba-get-bit child0 eba))
+                       (eql 1 (eba-get-bit child0 eba2)))
+                   (or (not (eql (id->type child1 aignet) (gate-type)))
+                       (eql 1 (eba-get-bit child1 eba))
+                       (eql 1 (eba-get-bit child1 eba2)))))
+      :const t
+      :in t
+      :out t)))
+
+
+(define any-lit-has-marked-children ((x lit-listp)
+                                     (eba)
+                                     (eba2)
+                                     (aignet))
+  :guard (and (aignet-lit-listp x aignet)
+              (< (max-fanin aignet) (eba-length eba))
+              (< (max-fanin aignet) (eba-length eba2)))
+  (if (atom x)
+      nil
+    (or (lit-has-marked-children (car x) eba eba2 aignet)
+        (any-lit-has-marked-children (cdr x) eba eba2 aignet))))
+      
+
+;; (define maybe-grow-truth4arr ((size natp) (truth4arr))
+;;   :returns (new-truth4arr)
+;;   (if (<= (lnfix size) (truth4s-length truth4arr))
+;;       truth4arr
+;;     (resize-truth4s (max 16 (* 2 (lnfix size))) truth4arr))
+;;   ///
+;;   (defret len-of-maybe-grow-truth4arr
+;;     (<= (nfix size) (len new-truth4arr))
+;;     :rule-classes :linear))
+
+
+(define aignet-and-if-not-redundant ((nlit litp)
+                                     (mlit litp)
+                                     (eba)
+                                     (eba2)
+                                     (truth4arr)
+                                     (truthmap truthmap-p)
+                                     (strash)
+                                     (aignet)
+                                     (lits-acc lit-listp))
+  :returns (mv (new-lits-acc lit-listp)
+               (new-eba)
+               (new-eba2)
+               (new-truthmap truthmap-p)
+               (new-truth4arr)
+               (new-strash)
+               (new-aignet))
+  :guard (and (fanin-litp nlit aignet)
+              (fanin-litp mlit aignet)
+              (aignet-truthmap-p truthmap aignet)
+              (< (max-fanin aignet) (eba-length eba))
+              (< (max-fanin aignet) (eba-length eba2))
+              (< (max-fanin aignet) (truth4s-length truth4arr)))
+  :prepwork (;; (local 
+             ;;        (defret num-nodes-of-aignet-install-and
+             ;;          (implies (not existing)
+             ;;                   (equal (node-count new-aignet) (+ 1 (node-count aignet))))
+             ;;          :hints(("Goal" :in-theory (enable aignet-install-and)))
+             ;;          :fn aignet-install-and))
+             ;; (local 
+             ;;        (defret aignet-litp-of-aignet-install-and
+             ;;          (implies (not existing)
+             ;;                   (aignet-litp lit new-aignet))
+             ;;          :hints(("Goal" :in-theory (enable aignet-install-and)))
+             ;;          :fn aignet-install-and))
+             ;; (local (def-aignet-preservation-thms aignet-install-and))
+             (local (in-theory (disable aignet-install-and-of-aignet-and-gate-simp/strash)))
+             (local (in-theory (enable aignet-install-and)))
+             )
+  (b* ((truthmap (truthmap-fix truthmap))
+       ((mv existing key lit1 lit2) (aignet-and-gate-simp/strash nlit mlit
+                                                                         9 strash aignet))
+       ((when existing)
+        (mv (lit-list-fix lits-acc)
+            eba eba2 truth4arr smm strash aignet))
+       (and-truth (logand (lit-truth nlit truth4arr)
+                          (lit-truth mlit truth4arr)))
+       (truth-lits (cdr (hons-get and-truth truthmap)))
+       ;; (ntruth-lits (len truth-lits))
+       ;; (- (and (< 100 ntruth-lits)
+       ;;         (cw "~x0: ~x1 lits~%" and-truth ntruth-lits)))
+       (neg-truth (truth-norm4 (lognot and-truth)))
+       (neg-truth-lits (cdr (hons-get neg-truth truthmap)))
+       ;; (nneg-truth-lits (len neg-truth-lits))
+       ;; (- (and (< 100 nneg-truth-lits)
+       ;;         (cw "~x0: ~x1 lits~%" neg-truth nneg-truth-lits)))
+       ((when (or (any-lit-has-marked-children
+                   truth-lits eba eba2 aignet)
+                  (any-lit-has-marked-children
+                   neg-truth-lits eba eba2 aignet)))
+        ;; (cw "~x0, ~x1: marked, skipping~%" nlit mlit)
+        (mv (lit-list-fix lits-acc)
+            eba eba2 truth4arr smm strash aignet))
+       (new-id (num-nodes aignet))
+       ((mv lit strash aignet) (aignet-install-and nil key lit1 lit2 strash aignet))
+       (truthmap (hons-acons and-truth (cons lit truth-lits) truthmap))
+       (truth4arr (maybe-grow-truth4arr new-id truth4arr))
+       (truth4arr (set-truth4 new-id and-truth truth4arr))
+       (eba (maybe-grow-eba new-id eba))
+       (eba2 (maybe-grow-eba new-id eba2)))
+    (mv (cons lit (lit-list-fix lits-acc))
+        eba eba2 truth4arr smm strash aignet))
+  ///
+  
+
+  (def-aignet-preservation-thms aignet-and-if-not-redundant :stobjname aignet)
+
+  (defret aignet-litp-of-aignet-and-if-not-redundant
+    (implies (and (aignet-litp nlit aignet)
+                  (aignet-litp mlit aignet)
+                  (aignet-lit-listp lits-acc aignet))
+             (aignet-lit-listp new-lits-acc new-aignet)))
+
+  (defret aignet-truthmap-p-of-aignet-and-if-not-redundant
+    (implies (aignet-truthmap-p truthmap aignet)
+             (aignet-truthmap-p new-truthmap new-aignet))
+    :hints (("goal" :expand ((:free (a b aignet) (aignet-truthmap-p (cons a b) aignet))))))
+
+  ;; (defret aignet-and-if-not-redundant-correct
+  ;;   (implies (and (aignet-litp nlit aignet)
+  ;;                 (aignet-litp mlit aignet)
+  ;;                 new-lit)
+  ;;            (equal (lit-eval new-lit invals regvals new-aignet)
+  ;;                   (eval-and-of-lits nlit mlit invals regvals aignet)))
+  ;;   :hints(("Goal" :expand ((:free (n aignet)
+  ;;                            (lit-eval (make-lit n 0) invals regvals aignet))))))
+
+  (defret truth4arr-length-of-aignet-and-if-not-redundant
+    (implies (< (node-count (find-max-fanin aignet)) (len truth4arr))
+             (< (node-count (find-max-fanin new-aignet)) (len new-truth4arr)))
+    :rule-classes (:rewrite (:linear :trigger-terms ((node-count (find-max-fanin new-aignet))
+                                                     (len new-truth4arr)))))
+
+  (defret eba-length-of-aignet-and-if-not-redundant
+    (implies (< (node-count (find-max-fanin aignet)) (len eba))
+             (< (node-count (find-max-fanin new-aignet)) (len new-eba)))
+    :rule-classes (:rewrite (:linear :trigger-terms ((node-count (find-max-fanin new-aignet))
+                                                     (len new-eba)))))
+
+  (defret eba2-length-of-aignet-and-if-not-redundant
+    (implies (< (node-count (find-max-fanin aignet)) (len eba2))
+             (< (node-count (find-max-fanin new-aignet)) (len new-eba2)))
+    :rule-classes (:rewrite (:linear :trigger-terms ((node-count (find-max-fanin new-aignet))
+                                                     (len new-eba2)))))
+
+  (defret stype-count-of-aignet-and-if-not-redundant
+    (implies (not (equal (stype-fix stype) :gate))
+             (equal (stype-count stype new-aignet)
+                    (stype-count stype aignet)))))
+       
+       
+
+(define aignet-ands-if-not-redundant ((n litp)
+                                      (m litp)
+                                      (eba "bit array marked with n's cone")
+                                      (eba2 "bit array to be marked with m's cone")
+                                      (truth4arr "truth values of aignet ids")
+                                      (truthmap truthmap-p "truth values to list of aignet lits")
+                                      (strash)
+                                      (aignet)
+                                      (lits-acc lit-listp))
+  :guard (and (fanin-litp n aignet)
+              (fanin-litp m aignet)
+              (aignet-truthmap-p truthmap aignet)
+              (< (max-fanin aignet) (eba-length eba))
+              (< (max-fanin aignet) (eba-length eba2))
+              (< (max-fanin aignet) (truth4s-length truth4arr)))
+  :guard-hints (("goal" :do-not-induct t))
+  :returns (mv (new-lits-acc lit-listp)
+               (new-eba)
+               (new-eba2)
+               (new-truthmap truthmap-p)
+               (new-truth4arr)
+               (new-strash)
+               (new-aignet))
+  :prepwork ((local (in-theory (disable len acl2::repeat-when-zp aignet-lit-listp
+                                        SATLINK::EQUAL-OF-LIT-NEGATE-COND-COMPONENT-REWRITES))))
+  (b* ((eba2 (eba-clear eba2))
+       (eba2 (aignet-mark-cone (lit-id m) eba2 aignet))
+       (~n (lit-negate n))
+       (~m (lit-negate m))
+       ((mv lits-acc eba eba2 truthmap truth4arr strash aignet)
+        (aignet-and-if-not-redundant n m eba eba2 truth4arr truthmap strash aignet lits-acc))
+       ((mv lits-acc eba eba2 truthmap truth4arr strash aignet)
+        (aignet-and-if-not-redundant n ~m eba eba2 truth4arr truthmap strash aignet lits-acc))
+       ((mv lits-acc eba eba2 truthmap truth4arr strash aignet)
+        (aignet-and-if-not-redundant ~n m eba eba2 truth4arr truthmap strash aignet lits-acc)))
+    (aignet-and-if-not-redundant ~n ~m eba eba2 truth4arr truthmap strash aignet lits-acc))
+  ///
+  
+  
+  (def-aignet-preservation-thms aignet-ands-if-not-redundant :stobjname aignet)
+
+  (defret aignet-litp-of-aignet-ands-if-not-redundant
+    (implies (and (aignet-litp n aignet)
+                  (aignet-litp m aignet)
+                  (aignet-lit-listp lits-acc aignet))
+             (aignet-lit-listp new-lits-acc new-aignet)))
+
+  (defret aignet-truthmap-p-of-aignet-ands-if-not-redundant
+    (implies (aignet-truthmap-p truthmap aignet)
+             (aignet-truthmap-p new-truthmap new-aignet))
+    :hints (("goal" :expand ((:free (a b aignet) (aignet-truthmap-p (cons a b) aignet))))))
+
+  (defret truth4arr-length-of-aignet-ands-if-not-redundant
+    (implies (< (node-count (find-max-fanin aignet)) (len truth4arr))
+             (< (node-count (find-max-fanin new-aignet)) (len new-truth4arr)))
+    :rule-classes :linear)
+
+  (defret eba-length-of-aignet-ands-if-not-redundant
+    (implies (< (node-count (find-max-fanin aignet)) (len eba))
+             (< (node-count (find-max-fanin new-aignet)) (len new-eba)))
+    :rule-classes :linear)
+
+  (defret eba2-length-of-aignet-ands-if-not-redundant
+    (implies (and (aignet-litp m aignet)
+                  (< (node-count (find-max-fanin aignet)) (len eba2)))
+             (< (node-count (find-max-fanin new-aignet)) (len new-eba2)))
+    ;; :rule-classes (:rewrite
+    ;;                (:linear :trigger-terms
+    ;;                 ((node-count (find-max-fanin new-aignet))
+    ;;                  (len new-eba2))))
+    :rule-classes :linear
+    )
+
+  (defret stype-count-of-aignet-ands-if-not-redundant
+    (implies (not (equal (stype-fix stype) :gate))
+             (equal (stype-count stype new-aignet)
+                    (stype-count stype aignet)))))
+
+
+(local (defthm stype-when-stype-count-0
+         (implies (and (aignet-extension-bind-inverse)
+                       (equal (stype-count stype new) 0)
+                       (not (equal (stype-fix stype) :const)))
+                  (not (equal (stype (car orig)) stype)))
+         :hints(("Goal" :in-theory (enable aignet-extension-p stype-count)))))
+
+
+(local (defthm aignet-litp-when-no-outs
+         (implies (and (equal (stype-count :po aignet) 0)
+                       (equal (stype-count :nxst aignet) 0))
+                  (equal (aignet-litp lit aignet)
+                         (< (lit-id lit) (num-nodes aignet))))
+         :hints(("Goal" :in-theory (enable aignet-litp ctype)
+                 :cases ((< (lit-id lit) (num-nodes aignet)))))))
+
+
+(define aignet-and-lits-with-node ((lit litp)
+                                   (lits lit-listp)
+                                   (eba "bit array marked with lit's cone")
+                                   (eba2 "bit array to be marked with lits' cone")
+                                   (truth4arr "truth values of aignet ids")
+                                   (truthmap truthmap-p "truth values to list of aignet lits")
+                                   (strash)
+                                   (aignet)
+                                   (lits-acc lit-listp))
+  :guard (and (aignet-lit-listp lits aignet)
+              (fanin-litp lit aignet)
+              (aignet-truthmap-p truthmap aignet)
+              (< (max-fanin aignet) (eba-length eba))
+              (< (max-fanin aignet) (eba-length eba2))
+              (< (max-fanin aignet) (truth4s-length truth4arr)))
+  :guard-hints (("goal" :do-not-induct t))
+  :returns (mv (new-lits-acc lit-listp)
+               (new-eba)
+               (new-eba2)
+               (new-truthmap truthmap-p)
+               (new-truth4arr)
+               (new-strash)
+               (new-aignet))
+  :measure (len lits)
+  (b* (((when (atom lits))
+        (mv (lit-list-fix lits-acc)
+            eba eba2 (truthmap-fix truthmap) truth4arr strash aignet))
+       ((mv lits-acc eba eba2 truthmap truth4arr strash aignet)
+        (aignet-ands-if-not-redundant
+         lit (car lits) eba eba2 truth4arr truthmap strash aignet lits-acc)))
+    (aignet-and-lits-with-node lit (cdr lits) eba eba2 truth4arr truthmap strash aignet lits-acc))
+  ///
+
+  
+  
+  (def-aignet-preservation-thms aignet-and-lits-with-node :stobjname aignet)
+
+  (defret aignet-litp-of-aignet-and-lits-with-node
+    (implies (and (aignet-litp lit aignet)
+                  (aignet-lit-listp lits aignet)
+                  (aignet-lit-listp lits-acc aignet))
+             (aignet-lit-listp new-lits-acc new-aignet))
+    :hints (("goal" :induct <call> :expand (<call>))))
+
+  (defret aignet-truthmap-p-of-aignet-and-lits-with-node
+    (implies (aignet-truthmap-p truthmap aignet)
+             (aignet-truthmap-p new-truthmap new-aignet))
+    :hints (("goal" :expand ((:free (a b aignet) (aignet-truthmap-p (cons a b) aignet))))))
+
+  (defret truth4arr-length-of-aignet-and-lits-with-node
+    (implies (< (node-count (find-max-fanin aignet)) (len truth4arr))
+             (< (node-count (find-max-fanin new-aignet)) (len new-truth4arr)))
+    :rule-classes (:rewrite (:linear :trigger-terms ((node-count (find-max-fanin new-aignet))
+                                                     (len new-truth4arr)))))
+
+  (defret eba-length-of-aignet-and-lits-with-node
+    (implies (< (node-count (find-max-fanin aignet)) (len eba))
+             (< (node-count (find-max-fanin new-aignet)) (len new-eba)))
+    :rule-classes (:rewrite (:linear :trigger-terms ((node-count (find-max-fanin new-aignet))
+                                                     (len new-eba)))))
+
+  (defret eba2-length-of-aignet-and-lits-with-node
+    (implies (and (aignet-lit-listp lits aignet)
+                  (< (node-count (find-max-fanin aignet)) (len eba2)))
+             (< (node-count (find-max-fanin new-aignet)) (len new-eba2)))
+    :hints (("goal" :induct <call> :expand (<call>)))
+    :rule-classes (:rewrite (:linear :trigger-terms ((node-count (find-max-fanin new-aignet))
+                                                     (len new-eba2)))))
+
+  (defret stype-count-of-aignet-and-lits-with-node
+    (implies (not (equal (stype-fix stype) :gate))
+             (equal (stype-count stype new-aignet)
+                    (stype-count stype aignet)))))
+
+
+
+
+(local (defthmd max-fanin-when-no-outs
+         (implies (and (equal (stype-count :po aignet) 0)
+                       (equal (stype-count :nxst aignet) 0))
+                  (equal (find-max-fanin aignet)
+                         (node-list-fix aignet)))
+         :hints(("Goal" :in-theory (enable find-max-fanin ctype)
+                 :expand ((find-max-fanin aignet))
+                 :do-not-induct t))))
+
+(define aignet-and-lits-with-nodes-up-to ((m posp)
+                                          (max-m posp)
+                                          (lits lit-listp)
+                                          (eba "bit array marked with n's cone")
+                                          (eba2 "bit array to be marked with m's cone")
+                                          (truth4arr "truth values of aignet ids")
+                                          (truthmap truthmap-p "truth values to list of aignet lits")
+                                          (strash)
+                                          (aignet)
+                                          (lits-acc lit-listp))
+  :guard (and (equal (num-outs aignet) 0)
+              (equal (num-nxsts aignet) 0)
+              (aignet-lit-listp lits aignet)
+              (<= max-m (num-nodes aignet))
+              (<= m max-m)
+              (aignet-truthmap-p truthmap aignet)
+              (< (max-fanin aignet) (eba-length eba))
+              (< (max-fanin aignet) (eba-length eba2))
+              (< (max-fanin aignet) (truth4s-length truth4arr)))
+  :guard-hints (("goal" :do-not-induct t)
+                (and stable-under-simplificationp
+                     '(:in-theory (enable max-fanin-when-no-outs))))
+  :returns (mv (new-lits-acc lit-listp)
+               (new-eba)
+               (new-eba2)
+               (new-truthmap truthmap-p)
+               (new-truth4arr)
+               (new-strash)
+               (new-aignet))
+  ;; :guard-debug t
+  :measure (nfix (- (lposfix max-m) (lposfix m)))
+  (b* (((when (mbe :logic (zp (- (lposfix max-m) (lposfix m)))
+                   :exec (eql m max-m)))
+        (mv (lit-list-fix lits-acc)
+            eba eba2 (truthmap-fix truthmap) truth4arr strash aignet))
+       (m (lposfix m))
+       (lit (mk-lit m 0))
+       (eba (eba-clear eba))
+       (eba (aignet-mark-cone m eba aignet))
+       ((mv lits-acc eba eba2 truthmap truth4arr strash aignet)
+        (aignet-and-lits-with-node
+         lit lits eba eba2 truth4arr truthmap strash aignet lits-acc)))
+    (aignet-and-lits-with-nodes-up-to (1+ (lposfix m)) max-m lits eba eba2 truth4arr truthmap strash aignet lits-acc))
+  ///
+
+  
+  
+  (def-aignet-preservation-thms aignet-and-lits-with-nodes-up-to :stobjname aignet)
+
+  (defret aignet-litp-of-aignet-and-lits-with-nodes-up-to
+    (implies (and (aignet-lit-listp lits aignet)
+                  (equal (stype-count :po aignet) 0)
+                  (equal (stype-count :nxst aignet) 0)
+                  (<= (lposfix max-m) (+ 1 (node-count aignet)))
+                  (aignet-lit-listp lits-acc aignet))
+             (aignet-lit-listp new-lits-acc new-aignet)))
+
+  (defret aignet-truthmap-p-of-aignet-and-lits-with-nodes-up-to
+    (implies (aignet-truthmap-p truthmap aignet)
+             (aignet-truthmap-p new-truthmap new-aignet))
+    :hints (("goal" :expand ((:free (a b aignet) (aignet-truthmap-p (cons a b) aignet))))))
+
+  (defret truth4arr-length-of-aignet-and-lits-with-nodes-up-to
+    (implies (< (node-count (find-max-fanin aignet)) (len truth4arr))
+             (< (node-count (find-max-fanin new-aignet)) (len new-truth4arr)))
+    :rule-classes (:rewrite (:linear :trigger-terms ((node-count (find-max-fanin new-aignet))
+                                                     (len new-truth4arr)))))
+
+  (local (defthm <=-max-fanin-when-<=-node-count
+           (implies (and (equal (stype-count :po aignet) 0)
+                         (equal (stype-count :nxst aignet) 0)
+                         (< n (+ 1 (node-count aignet)))
+                         (natp n))
+                    (<= n (node-count (find-max-fanin aignet))))
+           :hints(("Goal" :in-theory (enable max-fanin-when-no-outs)))))
+
+  (defret eba-length-of-aignet-and-lits-with-nodes-up-to
+    (implies (and (equal (stype-count :po aignet) 0)
+                  (equal (stype-count :nxst aignet) 0)
+                  (<= (lposfix max-m) (+ 1 (node-count aignet)))
+                  (< (node-count (find-max-fanin aignet)) (len eba)))
+             (< (node-count (find-max-fanin new-aignet)) (len new-eba)))
+    :hints (("Goal" :induct <call> :expand (<call>)))
+    :rule-classes (:rewrite (:linear :trigger-terms ((node-count (find-max-fanin new-aignet))
+                                                     (len new-eba)))))
+
+  (defret eba2-length-of-aignet-and-lits-with-nodes-up-to
+    (implies (and (aignet-lit-listp lits aignet)
+                  (< (node-count (find-max-fanin aignet)) (len eba2)))
+             (< (node-count (find-max-fanin new-aignet)) (len new-eba2)))
+    :rule-classes (:rewrite (:linear :trigger-terms ((node-count (find-max-fanin new-aignet))
+                                                     (len new-eba2)))))
+
+  (defret stype-count-of-aignet-and-lits-with-nodes-up-to
+    (implies (not (equal (stype-fix stype) :gate))
+             (equal (stype-count stype new-aignet)
+                    (stype-count stype aignet)))))
+
+;; (define aignet-and-lit-with-nodes-up-to ((m posp)
+;;                                          (max-m posp)
+;;                                          (lit litp)
+;;                                          (eba "bit array marked with n's cone")
+;;                                          (eba2 "bit array to be marked with m's cone")
+;;                                          (truth4arr "truth values of aignet ids")
+;;                                          (truthmap truthmap-p "truth values to list of aignet lits")
+;;                                          (strash)
+;;                                          (aignet)
+;;                                          (lits-acc lit-listp))
+;;   :guard (and (equal (num-outs aignet) 0)
+;;               (equal (num-nxsts aignet) 0)
+;;               (fanin-litp lit aignet)
+;;               (<= max-m (num-nodes aignet))
+;;               (<= m max-m)
+;;               (aignet-truthmap-p truthmap aignet)
+;;               (< (max-fanin aignet) (eba-length eba))
+;;               (< (max-fanin aignet) (eba-length eba2))
+;;               (< (max-fanin aignet) (truth4s-length truth4arr)))
+;;   :guard-hints (("goal" :do-not-induct t))
+;;   :returns (mv (new-lits-acc lit-listp)
+;;                (new-eba)
+;;                (new-eba2)
+;;                (new-truthmap truthmap-p)
+;;                (new-truth4arr)
+;;                (new-strash)
+;;                (new-aignet))
+;;   :measure (nfix (- (lposfix max-m) (lposfix m)))
+;;   (b* (((when (mbe :logic (zp (- (lposfix max-m) (lposfix m)))
+;;                    :exec (eql m max-m)))
+;;         (mv (lit-list-fix lits-acc)
+;;             eba eba2 (truthmap-fix truthmap) truth4arr strash aignet))
+;;        ((mv lits-acc eba eba2 truthmap truth4arr strash aignet)
+;;         (aignet-ands-if-not-redundant
+;;          lit (mk-lit (lposfix m) 0) eba eba2 truth4arr truthmap strash aignet lits-acc)))
+;;     (aignet-and-lit-with-nodes-up-to (1+ (lposfix m)) max-m lit eba eba2 truth4arr truthmap strash aignet lits-acc))
+;;   ///
+
+  
+  
+;;   (def-aignet-preservation-thms aignet-and-lit-with-nodes-up-to :stobjname aignet)
+
+;;   (defret aignet-litp-of-aignet-and-lit-with-nodes-up-to
+;;     (implies (and (aignet-litp lit aignet)
+;;                   (equal (stype-count :po aignet) 0)
+;;                   (equal (stype-count :nxst aignet) 0)
+;;                   (<= (lposfix max-m) (+ 1 (node-count aignet)))
+;;                   (aignet-lit-listp lits-acc aignet))
+;;              (aignet-lit-listp new-lits-acc new-aignet)))
+
+;;   (defret aignet-truthmap-p-of-aignet-and-lit-with-nodes-up-to
+;;     (implies (aignet-truthmap-p truthmap aignet)
+;;              (aignet-truthmap-p new-truthmap new-aignet))
+;;     :hints (("goal" :expand ((:free (a b aignet) (aignet-truthmap-p (cons a b) aignet))))))
+
+;;   (defret truth4arr-length-of-aignet-and-lit-with-nodes-up-to
+;;     (implies (< (node-count (find-max-fanin aignet)) (len truth4arr))
+;;              (< (node-count (find-max-fanin new-aignet)) (len new-truth4arr)))
+;;     :rule-classes (:rewrite (:linear :trigger-terms ((node-count (find-max-fanin new-aignet))
+;;                                                      (len new-truth4arr)))))
+
+;;   (defret eba-length-of-aignet-and-lit-with-nodes-up-to
+;;     (implies (< (node-count (find-max-fanin aignet)) (len eba))
+;;              (< (node-count (find-max-fanin new-aignet)) (len new-eba)))
+;;     :rule-classes (:rewrite (:linear :trigger-terms ((node-count (find-max-fanin new-aignet))
+;;                                                      (len new-eba)))))
+
+;;   (defret eba2-length-of-aignet-and-lit-with-nodes-up-to
+;;     (implies (and (equal (stype-count :po aignet) 0)
+;;                   (equal (stype-count :nxst aignet) 0)
+;;                   (<= (lposfix max-m) (+ 1 (node-count aignet)))
+;;                   (< (node-count (find-max-fanin aignet)) (len eba2)))
+;;              (< (node-count (find-max-fanin new-aignet)) (len new-eba2)))
+;;     :rule-classes (:rewrite (:linear :trigger-terms ((node-count (find-max-fanin new-aignet))
+;;                                                      (len new-eba2)))))
+
+;;   (defret stype-count-of-aignet-and-lit-with-nodes-up-to
+;;     (implies (not (equal (stype-fix stype) :gate))
+;;              (equal (stype-count stype new-aignet)
+;;                     (stype-count stype aignet)))))
+
+
+
+
+
+;; (define aignet-and-lits-with-nodes-up-to ((max-m posp)
+;;                                           (lits lit-listp)
+;;                                           (eba "bit array marked with n's cone")
+;;                                           (eba2 "bit array to be marked with m's cone")
+;;                                           (truth4arr "truth values of aignet ids")
+;;                                           (truthmap truthmap-p "truth values to list of aignet lits")
+;;                                           (strash)
+;;                                           (aignet)
+;;                                           (lits-acc lit-listp))
+;;   :guard (and (equal (num-outs aignet) 0)
+;;               (equal (num-nxsts aignet) 0)
+;;               (aignet-lit-listp lits aignet)
+;;               (<= max-m (num-nodes aignet))
+;;               (aignet-truthmap-p truthmap aignet)
+;;               (< (max-fanin aignet) (eba-length eba))
+;;               (< (max-fanin aignet) (eba-length eba2))
+;;               (< (max-fanin aignet) (truth4s-length truth4arr)))
+;;   :guard-hints (("goal" :do-not-induct t :expand ((aignet-lit-listp lits aignet)))
+;;                 (and stable-under-simplificationp
+;;                      '(:in-theory (enable max-fanin-when-no-outs))))
+;;   ;; :guard-debug t
+;;   :returns (mv (new-lits-acc lit-listp)
+;;                (new-eba)
+;;                (new-eba2)
+;;                (new-truthmap truthmap-p)
+;;                (new-truth4arr)
+;;                (new-strash)
+;;                (new-aignet))
+;;   :measure (len lits)
+;;   (b* (((when (atom lits))
+;;         (mv (lit-list-fix lits-acc)
+;;             eba eba2 (truthmap-fix truthmap) truth4arr strash aignet))
+;;        (eba (eba-clear eba))
+;;        (eba (aignet-mark-cone (lit-id (car lits)) eba aignet))
+;;        ((mv lits-acc eba eba2 truthmap truth4arr strash aignet)
+;;         (aignet-and-lit-with-nodes-up-to 1 max-m (car lits) eba eba2 truth4arr truthmap strash aignet lits-acc)))
+;;     (aignet-and-lits-with-nodes-up-to max-m (cdr lits) eba eba2 truth4arr truthmap strash aignet lits-acc))
+;;   ///
+
+    
+;;   (def-aignet-preservation-thms aignet-and-lits-with-nodes-up-to :stobjname aignet)
+
+;;   (defret aignet-litp-of-aignet-and-lits-with-nodes-up-to
+;;     (implies (and (aignet-lit-listp lits aignet)
+;;                   (equal (stype-count :po aignet) 0)
+;;                   (equal (stype-count :nxst aignet) 0)
+;;                   (<= (lposfix max-m) (+ 1 (node-count aignet)))
+;;                   (aignet-lit-listp lits-acc aignet))
+;;              (aignet-lit-listp new-lits-acc new-aignet))
+;;     :hints (("Goal" :induct <call> :expand (<call>))))
+
+;;   (defret aignet-truthmap-p-of-aignet-and-lits-with-nodes-up-to
+;;     (implies (aignet-truthmap-p truthmap aignet)
+;;              (aignet-truthmap-p new-truthmap new-aignet))
+;;     :hints (("goal" :expand ((:free (a b aignet) (aignet-truthmap-p (cons a b) aignet))))))
+
+;;   (defret truth4arr-length-of-aignet-and-lits-with-nodes-up-to
+;;     (implies (< (node-count (find-max-fanin aignet)) (len truth4arr))
+;;              (< (node-count (find-max-fanin new-aignet)) (len new-truth4arr)))
+;;     :rule-classes :linear)
+
+;;   (defret eba-length-of-aignet-and-lits-with-nodes-up-to
+;;     (implies (and (aignet-lit-listp lits aignet)
+;;                   (< (node-count (find-max-fanin aignet)) (len eba)))
+;;              (< (node-count (find-max-fanin new-aignet)) (len new-eba)))
+;;     :hints (("Goal" :induct <call> :expand (<call>)))
+;;     :rule-classes :linear)
+
+;;   (defret eba2-length-of-aignet-and-lits-with-nodes-up-to
+;;     (implies (and (equal (stype-count :po aignet) 0)
+;;                   (equal (stype-count :nxst aignet) 0)
+;;                   (<= (lposfix max-m) (+ 1 (node-count aignet)))
+;;                   (< (node-count (find-max-fanin aignet)) (len eba2)))
+;;              (< (node-count (find-max-fanin new-aignet)) (len new-eba2)))
+;;     :rule-classes :linear)
+
+;;   (defret stype-count-of-aignet-and-lits-with-nodes-up-to
+;;     (implies (not (equal (stype-fix stype) :gate))
+;;              (equal (stype-count stype new-aignet)
+;;                     (stype-count stype aignet)))))
+
+(define aignet-make-lit-products ((curr-level natp)
+                                  (max-level natp)
+                                  (prev-lits lit-listp)
+                                  (eba "bit array marked with n's cone")
+                                  (eba2 "bit array to be marked with m's cone")
+                                  (truth4arr "truth values of aignet ids")
+                                  (truthmap truthmap-p "truth values to list of aignet lits")
+                                  (strash)
+                                  (aignet))
+  :guard (and (equal (num-outs aignet) 0)
+              (equal (num-nxsts aignet) 0)
+              (aignet-lit-listp prev-lits aignet)
+              (aignet-truthmap-p truthmap aignet)
+              (<= curr-level max-level)
+              (< (max-fanin aignet) (eba-length eba))
+              (< (max-fanin aignet) (eba-length eba2))
+              (< (max-fanin aignet) (truth4s-length truth4arr)))
+  :guard-hints (("goal" :do-not-induct t :expand ((aignet-lit-listp lits aignet)))
+                (and stable-under-simplificationp
+                     '(:in-theory (enable max-fanin-when-no-outs))))
+  ;; :guard-debug t
+  :returns (mv ;; (new-lits lit-listp)
+               (new-eba)
+               (new-eba2)
+               (new-truthmap truthmap-p)
+               (new-truth4arr)
+               (new-strash)
+               (new-aignet))
+  :measure (nfix (- (nfix max-level) (nfix curr-level)))
+  (b* ((- (cw "Level ~x0: ~x1 new lits, ~x2 nodes total~%" curr-level
+              (len prev-lits) (num-nodes aignet)))
+       ((when (mbe :logic (zp (- (nfix max-level) (nfix curr-level)))
+                   :exec (eql max-level curr-level)))
+        (mv eba eba2 (truthmap-fix truthmap) truth4arr strash aignet))
+       (curr-nodes (num-nodes aignet))
+       ((mv next-lits eba eba2 truthmap truth4arr strash aignet)
+        (aignet-and-lits-with-nodes-up-to 1 curr-nodes prev-lits eba eba2 truth4arr truthmap strash aignet nil)))
+    (aignet-make-lit-products (1+ (lnfix curr-level)) max-level next-lits eba eba2 truth4arr truthmap strash aignet))
+  ///
+
+    
+  (def-aignet-preservation-thms aignet-make-lit-products :stobjname aignet)
+
+  (defret aignet-truthmap-p-of-aignet-make-lit-products
+    (implies (aignet-truthmap-p truthmap aignet)
+             (aignet-truthmap-p new-truthmap new-aignet))
+    :hints (("goal" :expand ((:free (a b aignet) (aignet-truthmap-p (cons a b) aignet))))))
+
+  (defret truth4arr-length-of-aignet-make-lit-products
+    (implies (< (node-count (find-max-fanin aignet)) (len truth4arr))
+             (< (node-count (find-max-fanin new-aignet)) (len new-truth4arr)))
+    :rule-classes :linear)
+
+  (defret eba-length-of-aignet-make-lit-products
+    (implies (and (aignet-lit-listp prev-lits aignet)
+                  (equal (stype-count :po aignet) 0)
+                  (equal (stype-count :nxst aignet) 0)
+                  (< (node-count (find-max-fanin aignet)) (len eba)))
+             (< (node-count (find-max-fanin new-aignet)) (len new-eba)))
+    :hints (("Goal" :induct <call> :expand (<call>)))
+    :rule-classes :linear)
+
+  (defret eba2-length-of-aignet-make-lit-products
+    (implies (and (aignet-lit-listp prev-lits aignet)
+                  (equal (stype-count :po aignet) 0)
+                  (equal (stype-count :nxst aignet) 0)
+                  (< (node-count (find-max-fanin aignet)) (len eba2)))
+             (< (node-count (find-max-fanin new-aignet)) (len new-eba2)))
+    :rule-classes :linear)
+
+  (defret stype-count-of-aignet-make-lit-products
+    (implies (not (equal (stype-fix stype) :gate))
+             (equal (stype-count stype new-aignet)
+                    (stype-count stype aignet)))))
+    
+       
+
+(define aignet-make-levels ((max-levels natp)
+                            (truth4arr)
+                            (aignet))
+  :returns (mv (new-truthmap truthmap-p)
+               (new-truth4arr)
+               (new-aignet))
+  :prepwork ((local (include-book "std/lists/resize-list" :dir :System))
+             (local (in-theory (disable (resize-eba) (resize-truth4s) (resize-list) (acl2::repeat)))))
+  (b* (((acl2::local-stobjs eba eba2 strash)
+        (mv eba eba2 truthmap truth4arr strash aignet))
+       (aignet (aignet-init 0 0 4 50000 aignet))
+       (truth4arr (resize-truth4s 1000 truth4arr))
+       (aignet (aignet-add-in aignet))
+       (aignet (aignet-add-in aignet))
+       (aignet (aignet-add-in aignet))
+       (aignet (aignet-add-in aignet))
+       (start-lits '(2 4 6 8)) ;; input lits
+       (truth4arr (set-truth4 0 0 truth4arr))
+       (truth4arr (set-truth4 1 (var4 0) truth4arr))
+       (truth4arr (set-truth4 2 (var4 1) truth4arr))
+       (truth4arr (set-truth4 3 (var4 2) truth4arr))
+       (truth4arr (set-truth4 4 (var4 3) truth4arr))
+       (truthmap nil)
+       (truthmap (hons-acons 0 '(0) truthmap))
+       (truthmap (hons-acons (var4 0) '(2) truthmap))
+       (truthmap (hons-acons (var4 1) '(4) truthmap))
+       (truthmap (hons-acons (var4 2) '(6) truthmap))
+       (truthmap (hons-acons (var4 3) '(8) truthmap))
+       (eba (resize-eba 1000 eba))
+       (eba2 (resize-eba 1000 eba2)))
+    (aignet-make-lit-products 0 max-levels start-lits eba eba2 truth4arr truthmap strash aignet))
+  ///
+  
+  (defret aignet-truthmap-p-of-aignet-make-levels
+    (aignet-truthmap-p new-truthmap new-aignet)
+    :hints (("goal" :expand ((:free (a b aignet) (aignet-truthmap-p (cons a b) aignet))))))
+
+  (defret truth4arr-length-of-aignet-make-levels
+    (< (node-count (find-max-fanin new-aignet)) (len new-truth4arr))
+    :rule-classes :linear)
+
+  (defret stype-count-of-aignet-make-levels
+    (and (equal (stype-count :pi new-aignet) 4)
+         (equal (stype-count :reg new-aignet) 0)
+         (equal (stype-count :po new-aignet) 0)
+         (equal (stype-count :nxst new-aignet) 0))))
+       
+                                     
+
+
+
+(include-book "std/util/defconsts" :dir :system)
+
+(defconsts (*truthmap* truth4arr aignet) (aignet-make-levels 3 truth4arr aignet))
+
+
+(define aignet-print-cone-rec ((n natp) eba aignet)
+  :guard (and (< n (num-nodes aignet))
+              (not (eql (id->type n aignet) (out-type)))
+              (< (nfix n) (eba-length eba)))
+  :returns (mv msg new-eba)
+  :measure (nfix n)
+  :verify-guards nil
+  :prepwork ((local (in-theory (disable lookup-id-in-bounds-when-positive
+                                        lookup-id-out-of-bounds))))
+  (b* (((when (eql 1 (eba-get-bit n eba))) (mv "" eba))
+       (eba (eba-set-bit n eba))
+       ((unless (eql (id->type n aignet) (gate-type)))
+        (mv "" eba))
+       (msg (aignet-print-gate n aignet))
+       ((mv msg0 eba) (aignet-print-cone-rec (lit-id (gate-id->fanin0 n aignet)) eba aignet))
+       ((mv msg1 eba) (aignet-print-cone-rec (lit-id (gate-id->fanin1 n aignet)) eba aignet)))
+    (mv (acl2::msg "~@0~@1~@2~%" msg0 msg1 msg) eba))
+  ///
+  (defret eba-len-of-aignet-print-cone-rec
+    (implies (< (nfix n) (len eba))
+             (equal (len new-eba) (len eba))))
+  (verify-guards aignet-print-cone-rec
+    :hints(("Goal" :in-theory (enable aignet-idp)))))
+
+
+(define aignet-print-cone ((n natp) aignet)
+  :guard (and (< n (num-nodes aignet))
+              (not (eql (id->type n aignet) (out-type))))
+  :prepwork ((local (in-theory (enable aignet-idp))))
+  (b* (((acl2::local-stobjs eba)
+        (mv null eba))
+       (eba (resize-eba (+ 1 (nfix n)) eba))
+       ((mv msg eba) (aignet-print-cone-rec n eba aignet)))
+    (cw "~@0~%" msg)
+    (mv nil eba)))
+
+
+#!truth
+(define dsdlib-print-cone ((n natp) dsdlib)
+  :guard-hints (("goal" :in-theory (enable aignet::aignet-idp)))
+  (b* ((n (lnfix n)))
+    (stobj-let ((aignet (dsdlib->aigs dsdlib)))
+               (ans)
+               (and (< n (aignet::num-nodes aignet))
+                    (not (eql (aignet::id->type n aignet) (aignet::out-type)))
+                    (aignet::aignet-print-cone n aignet))
+               ans)))
+
+
+(define aignet-print-lit-cones ((lits lit-listp)
+                                (aignet))
+  :guard (aignet-lit-listp lits aignet)
+  (if (atom lits)
+      nil
+    (progn$ (aignet-print-cone (lit-id (car lits)) aignet)
+            (aignet-print-lit-cones (cdr lits) aignet))))
